Experiments/Test_Suite_Calculation.thy
@@ -228,14 +228,12 @@ in (Test_Suite nodes_with_preambles (fst tps_and_targets) (snd tps_and_targets) 
 
 
 
-
-definition calculate_test_suite_example :: "('a::linorder,'b::linorder,'c::linorder) fsm \<Rightarrow> nat \<Rightarrow> ('a,'b,'c, ('a \<times> 'a) + 'a) test_suite" where
-  "calculate_test_suite_example M m = 
+definition calculate_test_suite_for_repetition_sets :: "('a::linorder,'b::linorder,'c::linorder) fsm \<Rightarrow> nat \<Rightarrow> ('a set \<times> 'a set) list \<Rightarrow> ('a,'b,'c, ('a \<times> 'a) + 'a) test_suite" where
+  "calculate_test_suite_for_repetition_sets M m repetition_sets = 
     (let
          nodes_with_preambles = d_reachable_states_with_preambles M;
-         pairs_with_separators = image (\<lambda>((q1,q2),A) . ((q1,q2),A,Inr q1,Inr q2)) (r_distinguishable_state_pairs_with_separators M);
-         repetition_sets = maximal_repetition_sets_from_separators_list M
-  in combine_test_suite M m nodes_with_preambles pairs_with_separators repetition_sets)" 
+         pairs_with_separators = image (\<lambda>((q1,q2),A) . ((q1,q2),A,Inr q1,Inr q2)) (r_distinguishable_state_pairs_with_separators M)
+  in combine_test_suite M m nodes_with_preambles pairs_with_separators repetition_sets)"
 
 
 
@@ -289,15 +287,18 @@ qed
 
 subsection \<open>Sufficiency of the Calculated Test Suite\<close>
 
-lemma calculate_test_suite_example_sufficient_and_finite :
+lemma calculate_test_suite_for_repetition_sets_sufficient_and_finite :
   fixes M :: "('a::linorder,'b::linorder,'c::linorder) fsm"
   assumes "observable M"
   and     "completely_specified M"
   and     "inputs M \<noteq> {}"
-shows "is_sufficient_for_reduction_testing (calculate_test_suite_example M m) M m"
-and   "is_finite_test_suite (calculate_test_suite_example M m)"
+  and     "\<And>q. q \<in> FSM.nodes M \<Longrightarrow> \<exists>d\<in>set RepSets. q \<in> fst d"
+  and     "\<And>d. d \<in> set RepSets \<Longrightarrow> fst d \<subseteq> nodes M \<and> (snd d = fst d \<inter> fst ` d_reachable_states_with_preambles M)" 
+  and     "\<And> q1 q2 d. d \<in> set RepSets \<Longrightarrow> q1\<in>fst d \<Longrightarrow> q2\<in>fst d \<Longrightarrow> q1 \<noteq> q2 \<Longrightarrow> (q1, q2) \<in> fst ` r_distinguishable_state_pairs_with_separators M"
+shows "is_sufficient_for_reduction_testing (calculate_test_suite_for_repetition_sets M m RepSets) M m"
+and   "is_finite_test_suite (calculate_test_suite_for_repetition_sets M m RepSets)"
 proof -
-  obtain nodes_with_preambles tps rd_targets atcs where "calculate_test_suite_example M m = Test_Suite nodes_with_preambles tps rd_targets atcs"
+  obtain nodes_with_preambles tps rd_targets atcs where "calculate_test_suite_for_repetition_sets M m RepSets = Test_Suite nodes_with_preambles tps rd_targets atcs"
     using test_suite.exhaust by blast
 
   have "\<And> a b c d . Test_Suite nodes_with_preambles tps rd_targets atcs = Test_Suite a b c d \<Longrightarrow> tps = b"
@@ -306,41 +307,41 @@ proof -
   have nodes_with_preambles_def : "nodes_with_preambles = d_reachable_states_with_preambles M"
     
   
-  and tps_def                   : "tps = (\<lambda>q. (m2f_by \<Union> (set_as_map ((\<lambda>(q, p). (q, fst ` p)) ` (\<lambda>q. (q, m_traversal_paths_with_witness M q (maximal_repetition_sets_from_separators_list M) m)) ` fst ` d_reachable_states_with_preambles M))) q
+  and tps_def                   : "tps = (\<lambda>q. (m2f_by \<Union> (set_as_map ((\<lambda>(q, p). (q, fst ` p)) ` (\<lambda>q. (q, m_traversal_paths_with_witness M q RepSets m)) ` fst ` d_reachable_states_with_preambles M))) q
                                             \<union> (m2f (set_as_map ((\<lambda>(q, p, q'). (q, p)) `
-                                                ((\<Union>q\<in>fst ` d_reachable_states_with_preambles M. \<Union> (prefix_pair_tests q ` (m2f (set_as_map ((\<lambda>q. (q, m_traversal_paths_with_witness M q (maximal_repetition_sets_from_separators_list M) m)) ` fst ` d_reachable_states_with_preambles M)) q))) 
-                                                \<union> (\<Union>q\<in>fst ` d_reachable_states_with_preambles M. \<Union>mrsps\<in> m2f (set_as_map ((\<lambda>q. (q, m_traversal_paths_with_witness M q (maximal_repetition_sets_from_separators_list M) m)) ` fst ` d_reachable_states_with_preambles M)) q . preamble_prefix_tests q mrsps (fst ` d_reachable_states_with_preambles M)) 
-                                                \<union> preamble_pair_tests (\<Union>(q, y)\<in>(\<lambda>q. (q, m_traversal_paths_with_witness M q (maximal_repetition_sets_from_separators_list M) m)) ` fst ` d_reachable_states_with_preambles M. (\<lambda>(p, rd, dr). dr) ` y) (fst ` (\<lambda>((q1, q2), A). ((q1, q2), A, Inr q1 :: 'a \<times> 'a + 'a, Inr q2 :: 'a \<times> 'a + 'a)) ` r_distinguishable_state_pairs_with_separators M))))) q)"
+                                                ((\<Union>q\<in>fst ` d_reachable_states_with_preambles M. \<Union> (prefix_pair_tests q ` (m2f (set_as_map ((\<lambda>q. (q, m_traversal_paths_with_witness M q RepSets m)) ` fst ` d_reachable_states_with_preambles M)) q))) 
+                                                \<union> (\<Union>q\<in>fst ` d_reachable_states_with_preambles M. \<Union>mrsps\<in> m2f (set_as_map ((\<lambda>q. (q, m_traversal_paths_with_witness M q RepSets m)) ` fst ` d_reachable_states_with_preambles M)) q . preamble_prefix_tests q mrsps (fst ` d_reachable_states_with_preambles M)) 
+                                                \<union> preamble_pair_tests (\<Union>(q, y)\<in>(\<lambda>q. (q, m_traversal_paths_with_witness M q RepSets m)) ` fst ` d_reachable_states_with_preambles M. (\<lambda>(p, rd, dr). dr) ` y) (fst ` (\<lambda>((q1, q2), A). ((q1, q2), A, Inr q1 :: 'a \<times> 'a + 'a, Inr q2 :: 'a \<times> 'a + 'a)) ` r_distinguishable_state_pairs_with_separators M))))) q)"
   and rd_targets_def            : "rd_targets = m2f (set_as_map
                                               ((\<lambda>(q, p, y). ((q, p), y)) `
-                                               ((\<Union>q\<in>fst ` d_reachable_states_with_preambles M. \<Union> (prefix_pair_tests q ` (m2f (set_as_map ((\<lambda>q. (q, m_traversal_paths_with_witness M q (maximal_repetition_sets_from_separators_list M) m)) ` fst ` d_reachable_states_with_preambles M)) q))) 
-                                               \<union> (\<Union>q\<in>fst ` d_reachable_states_with_preambles M. \<Union>mrsps\<in> m2f (set_as_map ((\<lambda>q. (q, m_traversal_paths_with_witness M q (maximal_repetition_sets_from_separators_list M) m)) ` fst ` d_reachable_states_with_preambles M)) q . preamble_prefix_tests q mrsps (fst ` d_reachable_states_with_preambles M)) 
-                                               \<union> preamble_pair_tests (\<Union>(q, y)\<in>(\<lambda>q. (q, m_traversal_paths_with_witness M q (maximal_repetition_sets_from_separators_list M) m)) ` fst ` d_reachable_states_with_preambles M. (\<lambda>(p, rd, dr). dr) ` y) (fst ` (\<lambda>((q1, q2), A). ((q1, q2), A, Inr q1 :: 'a \<times> 'a + 'a, Inr q2 :: 'a \<times> 'a + 'a)) ` r_distinguishable_state_pairs_with_separators M))))"
+                                               ((\<Union>q\<in>fst ` d_reachable_states_with_preambles M. \<Union> (prefix_pair_tests q ` (m2f (set_as_map ((\<lambda>q. (q, m_traversal_paths_with_witness M q RepSets m)) ` fst ` d_reachable_states_with_preambles M)) q))) 
+                                               \<union> (\<Union>q\<in>fst ` d_reachable_states_with_preambles M. \<Union>mrsps\<in> m2f (set_as_map ((\<lambda>q. (q, m_traversal_paths_with_witness M q RepSets m)) ` fst ` d_reachable_states_with_preambles M)) q . preamble_prefix_tests q mrsps (fst ` d_reachable_states_with_preambles M)) 
+                                               \<union> preamble_pair_tests (\<Union>(q, y)\<in>(\<lambda>q. (q, m_traversal_paths_with_witness M q RepSets m)) ` fst ` d_reachable_states_with_preambles M. (\<lambda>(p, rd, dr). dr) ` y) (fst ` (\<lambda>((q1, q2), A). ((q1, q2), A, Inr q1 :: 'a \<times> 'a + 'a, Inr q2 :: 'a \<times> 'a + 'a)) ` r_distinguishable_state_pairs_with_separators M))))"
   and  atcs_def                 : "atcs = m2f (set_as_map ((\<lambda>((q1, q2), A). ((q1, q2), A, Inr q1, Inr q2)) ` r_distinguishable_state_pairs_with_separators M))"
-    using \<open>calculate_test_suite_example M m = Test_Suite nodes_with_preambles tps rd_targets atcs\<close>[symmetric]
-    unfolding calculate_test_suite_example_def combine_test_suite_def Let_def calculate_test_paths_def fst_conv snd_conv by force+
+    using \<open>calculate_test_suite_for_repetition_sets M m RepSets = Test_Suite nodes_with_preambles tps rd_targets atcs\<close>[symmetric]
+    unfolding calculate_test_suite_for_repetition_sets_def combine_test_suite_def Let_def calculate_test_paths_def fst_conv snd_conv by force+
   
 
 
 
 
   have tps_alt_def: "\<And> q . q \<in> fst ` d_reachable_states_with_preambles M \<Longrightarrow> 
-          tps q = (fst ` m_traversal_paths_with_witness M q (maximal_repetition_sets_from_separators_list M) m) \<union> 
+          tps q = (fst ` m_traversal_paths_with_witness M q RepSets m) \<union> 
                   {z. (q, z)
                     \<in> (\<lambda>(q, p, q'). (q, p)) `
-                       ((prefix_pair_tests q (m_traversal_paths_with_witness M q (maximal_repetition_sets_from_separators_list M) m)) \<union>
+                       ((prefix_pair_tests q (m_traversal_paths_with_witness M q RepSets m)) \<union>
                         (\<Union>q\<in>fst ` d_reachable_states_with_preambles M.
-                            \<Union>mrsps\<in>{m_traversal_paths_with_witness M q (maximal_repetition_sets_from_separators_list M) m}.
+                            \<Union>mrsps\<in>{m_traversal_paths_with_witness M q RepSets m}.
                                preamble_prefix_tests q mrsps (fst ` d_reachable_states_with_preambles M)) \<union>
-                        preamble_pair_tests (\<Union>(q, y)\<in>(\<lambda>q. (q, m_traversal_paths_with_witness M q (maximal_repetition_sets_from_separators_list M) m)) ` fst ` d_reachable_states_with_preambles M. (\<lambda>(p, rd, dr). dr) ` y) (fst ` (\<lambda>((q1, q2), A). ((q1, q2), A, Inr q1 :: 'a \<times> 'a + 'a, Inr q2 :: 'a \<times> 'a + 'a)) ` r_distinguishable_state_pairs_with_separators M))}"
+                        preamble_pair_tests (\<Union>(q, y)\<in>(\<lambda>q. (q, m_traversal_paths_with_witness M q RepSets m)) ` fst ` d_reachable_states_with_preambles M. (\<lambda>(p, rd, dr). dr) ` y) (fst ` (\<lambda>((q1, q2), A). ((q1, q2), A, Inr q1 :: 'a \<times> 'a + 'a, Inr q2 :: 'a \<times> 'a + 'a)) ` r_distinguishable_state_pairs_with_separators M))}"
   and rd_targets_alt_def: "\<And> q p . q \<in> fst ` d_reachable_states_with_preambles M \<Longrightarrow> 
           rd_targets (q,p) = {z. ((q, p), z)
                    \<in> (\<lambda>(q, p, y). ((q, p), y)) `
-                      ((prefix_pair_tests q (m_traversal_paths_with_witness M q (maximal_repetition_sets_from_separators_list M) m)) \<union>
+                      ((prefix_pair_tests q (m_traversal_paths_with_witness M q RepSets m)) \<union>
                        (\<Union>q\<in>fst ` d_reachable_states_with_preambles M.
-                           \<Union>mrsps\<in>{m_traversal_paths_with_witness M q (maximal_repetition_sets_from_separators_list M) m}.
+                           \<Union>mrsps\<in>{m_traversal_paths_with_witness M q RepSets m}.
                               preamble_prefix_tests q mrsps (fst ` d_reachable_states_with_preambles M)) \<union>
-                       preamble_pair_tests (\<Union>(q, y)\<in>(\<lambda>q. (q, m_traversal_paths_with_witness M q (maximal_repetition_sets_from_separators_list M) m)) ` fst ` d_reachable_states_with_preambles M. (\<lambda>(p, rd, dr). dr) ` y) (fst ` (\<lambda>((q1, q2), A). ((q1, q2), A, Inr q1 :: 'a \<times> 'a + 'a, Inr q2 :: 'a \<times> 'a + 'a)) ` r_distinguishable_state_pairs_with_separators M))}"
+                       preamble_pair_tests (\<Union>(q, y)\<in>(\<lambda>q. (q, m_traversal_paths_with_witness M q RepSets m)) ` fst ` d_reachable_states_with_preambles M. (\<lambda>(p, rd, dr). dr) ` y) (fst ` (\<lambda>((q1, q2), A). ((q1, q2), A, Inr q1 :: 'a \<times> 'a + 'a, Inr q2 :: 'a \<times> 'a + 'a)) ` r_distinguishable_state_pairs_with_separators M))}"
   proof -
     fix q p assume "q \<in> fst ` d_reachable_states_with_preambles M"
 
@@ -348,15 +349,15 @@ proof -
 
     have scheme0 : "(case set_as_map
              ((\<lambda>(q, p). (q, fst ` p)) `
-              (\<lambda>q. (q, m_traversal_paths_with_witness M q (maximal_repetition_sets_from_separators_list M) m)) `
+              (\<lambda>q. (q, m_traversal_paths_with_witness M q RepSets m)) `
               fst ` d_reachable_states_with_preambles M)
              q of
-       None \<Rightarrow> \<Union> {} | Some x \<Rightarrow> \<Union> x) = image fst (m_traversal_paths_with_witness M q (maximal_repetition_sets_from_separators_list M) m)"
+       None \<Rightarrow> \<Union> {} | Some x \<Rightarrow> \<Union> x) = image fst (m_traversal_paths_with_witness M q RepSets m)"
     proof -
       have *: "((\<lambda>(q, p). (q, fst ` p)) `
-              (\<lambda>q. (q, m_traversal_paths_with_witness M q (maximal_repetition_sets_from_separators_list M) m)) `
+              (\<lambda>q. (q, m_traversal_paths_with_witness M q RepSets m)) `
               fst ` d_reachable_states_with_preambles M)
-               = (\<lambda> q . (q , image fst (m_traversal_paths_with_witness M q (maximal_repetition_sets_from_separators_list M) m))) ` (fst ` d_reachable_states_with_preambles M)"
+               = (\<lambda> q . (q , image fst (m_traversal_paths_with_witness M q RepSets m))) ` (fst ` d_reachable_states_with_preambles M)"
         by force
       have **: "\<And> f q xs . (case set_as_map
                               ((\<lambda>q. (q, f q)) ` xs)
@@ -381,16 +382,16 @@ proof -
     have scheme2: "(\<Union>q\<in>fst ` d_reachable_states_with_preambles M.
                    \<Union> (prefix_pair_tests q `
                        (if q \<in> fst ` d_reachable_states_with_preambles M
-                        then {m_traversal_paths_with_witness M q (maximal_repetition_sets_from_separators_list M) m} else {})))
-      = (\<Union>q\<in>fst ` d_reachable_states_with_preambles M. (\<Union> (prefix_pair_tests q ` {m_traversal_paths_with_witness M q (maximal_repetition_sets_from_separators_list M) m})))"
+                        then {m_traversal_paths_with_witness M q RepSets m} else {})))
+      = (\<Union>q\<in>fst ` d_reachable_states_with_preambles M. (\<Union> (prefix_pair_tests q ` {m_traversal_paths_with_witness M q RepSets m})))"
       unfolding set_as_map_def by auto
 
 
     have scheme3: "(\<Union>q\<in>fst ` d_reachable_states_with_preambles M.
                    \<Union>mrsps\<in>if q \<in> fst ` d_reachable_states_with_preambles M
-                           then {m_traversal_paths_with_witness M q (maximal_repetition_sets_from_separators_list M) m} else {}.
+                           then {m_traversal_paths_with_witness M q RepSets m} else {}.
                       preamble_prefix_tests q mrsps (fst ` d_reachable_states_with_preambles M))
-      = (\<Union>q\<in>fst ` d_reachable_states_with_preambles M. (\<Union>mrsps\<in>{m_traversal_paths_with_witness M q (maximal_repetition_sets_from_separators_list M) m} . preamble_prefix_tests q mrsps (fst ` d_reachable_states_with_preambles M)))"
+      = (\<Union>q\<in>fst ` d_reachable_states_with_preambles M. (\<Union>mrsps\<in>{m_traversal_paths_with_witness M q RepSets m} . preamble_prefix_tests q mrsps (fst ` d_reachable_states_with_preambles M)))"
       unfolding set_as_map_def by auto
 
     have scheme4 : "(fst ` (\<lambda>((q1, q2), A). ((q1, q2), A, Inr q1, Inr q2)) ` r_distinguishable_state_pairs_with_separators M)
@@ -401,15 +402,15 @@ proof -
     
 
 
-    have *:"tps q = (fst ` m_traversal_paths_with_witness M q (maximal_repetition_sets_from_separators_list M) m) \<union> 
+    have *:"tps q = (fst ` m_traversal_paths_with_witness M q RepSets m) \<union> 
                   {z. (q, z)
                     \<in> (\<lambda>(q, p, q'). (q, p)) `
                        ((\<Union>q\<in>fst ` d_reachable_states_with_preambles M.
-                            \<Union> (prefix_pair_tests q ` {m_traversal_paths_with_witness M q (maximal_repetition_sets_from_separators_list M) m})) \<union>
+                            \<Union> (prefix_pair_tests q ` {m_traversal_paths_with_witness M q RepSets m})) \<union>
                         (\<Union>q\<in>fst ` d_reachable_states_with_preambles M.
-                            \<Union>mrsps\<in>{m_traversal_paths_with_witness M q (maximal_repetition_sets_from_separators_list M) m}.
+                            \<Union>mrsps\<in>{m_traversal_paths_with_witness M q RepSets m}.
                                preamble_prefix_tests q mrsps (fst ` d_reachable_states_with_preambles M)) \<union>
-                        preamble_pair_tests (\<Union>(q, y)\<in>(\<lambda>q. (q, m_traversal_paths_with_witness M q (maximal_repetition_sets_from_separators_list M) m)) ` fst ` d_reachable_states_with_preambles M. (\<lambda>(p, rd, dr). dr) ` y) (fst ` (\<lambda>((q1, q2), A). ((q1, q2), A, Inr q1 :: 'a \<times> 'a + 'a, Inr q2 :: 'a \<times> 'a + 'a)) ` r_distinguishable_state_pairs_with_separators M))}"
+                        preamble_pair_tests (\<Union>(q, y)\<in>(\<lambda>q. (q, m_traversal_paths_with_witness M q RepSets m)) ` fst ` d_reachable_states_with_preambles M. (\<lambda>(p, rd, dr). dr) ` y) (fst ` (\<lambda>((q1, q2), A). ((q1, q2), A, Inr q1 :: 'a \<times> 'a + 'a, Inr q2 :: 'a \<times> 'a + 'a)) ` r_distinguishable_state_pairs_with_separators M))}"
       unfolding tps_def 
       unfolding scheme0 scheme1 scheme2 scheme3 scheme4
       unfolding set_as_map_def
@@ -422,47 +423,47 @@ proof -
     have **: "{z. (q, z)
                     \<in> (\<lambda>(q, p, q'). (q, p)) `
                        ((\<Union>q\<in>fst ` d_reachable_states_with_preambles M.
-                            \<Union> (prefix_pair_tests q ` {m_traversal_paths_with_witness M q (maximal_repetition_sets_from_separators_list M) m})) \<union>
+                            \<Union> (prefix_pair_tests q ` {m_traversal_paths_with_witness M q RepSets m})) \<union>
                         (\<Union>q\<in>fst ` d_reachable_states_with_preambles M.
-                            \<Union>mrsps\<in>{m_traversal_paths_with_witness M q (maximal_repetition_sets_from_separators_list M) m}.
+                            \<Union>mrsps\<in>{m_traversal_paths_with_witness M q RepSets m}.
                                preamble_prefix_tests q mrsps (fst ` d_reachable_states_with_preambles M)) \<union>
-                        preamble_pair_tests (\<Union>(q, y)\<in>(\<lambda>q. (q, m_traversal_paths_with_witness M q (maximal_repetition_sets_from_separators_list M) m)) ` fst ` d_reachable_states_with_preambles M. (\<lambda>(p, rd, dr). dr) ` y) (fst ` (\<lambda>((q1, q2), A). ((q1, q2), A, Inr q1 :: 'a \<times> 'a + 'a, Inr q2 :: 'a \<times> 'a + 'a)) ` r_distinguishable_state_pairs_with_separators M))}
+                        preamble_pair_tests (\<Union>(q, y)\<in>(\<lambda>q. (q, m_traversal_paths_with_witness M q RepSets m)) ` fst ` d_reachable_states_with_preambles M. (\<lambda>(p, rd, dr). dr) ` y) (fst ` (\<lambda>((q1, q2), A). ((q1, q2), A, Inr q1 :: 'a \<times> 'a + 'a, Inr q2 :: 'a \<times> 'a + 'a)) ` r_distinguishable_state_pairs_with_separators M))}
           = {z. (q, z)
                     \<in> (\<lambda>(q, p, q'). (q, p)) `
-                       ((prefix_pair_tests q (m_traversal_paths_with_witness M q (maximal_repetition_sets_from_separators_list M) m)) \<union>
+                       ((prefix_pair_tests q (m_traversal_paths_with_witness M q RepSets m)) \<union>
                         (\<Union>q\<in>fst ` d_reachable_states_with_preambles M.
-                            \<Union>mrsps\<in>{m_traversal_paths_with_witness M q (maximal_repetition_sets_from_separators_list M) m}.
+                            \<Union>mrsps\<in>{m_traversal_paths_with_witness M q RepSets m}.
                                preamble_prefix_tests q mrsps (fst ` d_reachable_states_with_preambles M)) \<union>
-                        preamble_pair_tests (\<Union>(q, y)\<in>(\<lambda>q. (q, m_traversal_paths_with_witness M q (maximal_repetition_sets_from_separators_list M) m)) ` fst ` d_reachable_states_with_preambles M. (\<lambda>(p, rd, dr). dr) ` y) (fst ` (\<lambda>((q1, q2), A). ((q1, q2), A, Inr q1 :: 'a \<times> 'a + 'a, Inr q2 :: 'a \<times> 'a + 'a)) ` r_distinguishable_state_pairs_with_separators M))}" 
+                        preamble_pair_tests (\<Union>(q, y)\<in>(\<lambda>q. (q, m_traversal_paths_with_witness M q RepSets m)) ` fst ` d_reachable_states_with_preambles M. (\<lambda>(p, rd, dr). dr) ` y) (fst ` (\<lambda>((q1, q2), A). ((q1, q2), A, Inr q1 :: 'a \<times> 'a + 'a, Inr q2 :: 'a \<times> 'a + 'a)) ` r_distinguishable_state_pairs_with_separators M))}" 
       (is "{z. (q, z) \<in> ?S1} = {z. (q, z) \<in> ?S2}")
     proof -
       have "\<And> z . (q, z) \<in> ?S1 \<Longrightarrow> (q, z) \<in> ?S2"
       proof -
         fix z assume "(q, z) \<in> ?S1"
         then consider "(q, z) \<in> (\<lambda>(q, p, q'). (q, p)) ` (\<Union>q\<in>fst ` d_reachable_states_with_preambles M.
-                            \<Union> (prefix_pair_tests q ` {m_traversal_paths_with_witness M q (maximal_repetition_sets_from_separators_list M) m}))"
+                            \<Union> (prefix_pair_tests q ` {m_traversal_paths_with_witness M q RepSets m}))"
                     | "(q,z) \<in> (\<lambda>(q, p, q'). (q, p)) `  (\<Union>q\<in>fst ` d_reachable_states_with_preambles M.
-                            \<Union>mrsps\<in>{m_traversal_paths_with_witness M q (maximal_repetition_sets_from_separators_list M) m}.
+                            \<Union>mrsps\<in>{m_traversal_paths_with_witness M q RepSets m}.
                                preamble_prefix_tests q mrsps (fst ` d_reachable_states_with_preambles M))"
-                    | "(q,z) \<in> (\<lambda>(q, p, q'). (q, p)) ` (preamble_pair_tests (\<Union>(q, y)\<in>(\<lambda>q. (q, m_traversal_paths_with_witness M q (maximal_repetition_sets_from_separators_list M) m)) ` fst ` d_reachable_states_with_preambles M. (\<lambda>(p, rd, dr). dr) ` y) (fst ` (\<lambda>((q1, q2), A). ((q1, q2), A, Inr q1 :: 'a \<times> 'a + 'a, Inr q2 :: 'a \<times> 'a + 'a)) ` r_distinguishable_state_pairs_with_separators M))"
+                    | "(q,z) \<in> (\<lambda>(q, p, q'). (q, p)) ` (preamble_pair_tests (\<Union>(q, y)\<in>(\<lambda>q. (q, m_traversal_paths_with_witness M q RepSets m)) ` fst ` d_reachable_states_with_preambles M. (\<lambda>(p, rd, dr). dr) ` y) (fst ` (\<lambda>((q1, q2), A). ((q1, q2), A, Inr q1 :: 'a \<times> 'a + 'a, Inr q2 :: 'a \<times> 'a + 'a)) ` r_distinguishable_state_pairs_with_separators M))"
           by blast
         then show "(q, z) \<in> ?S2" proof cases
           case 1
           have scheme: "\<And> f y xs . y \<in> image f xs \<Longrightarrow> \<exists> x . x \<in> xs \<and> f x = y" by auto
 
-          obtain qzq where "qzq \<in> (\<Union>q\<in>fst ` d_reachable_states_with_preambles M. \<Union> (prefix_pair_tests q ` {m_traversal_paths_with_witness M q (maximal_repetition_sets_from_separators_list M) m}))"
+          obtain qzq where "qzq \<in> (\<Union>q\<in>fst ` d_reachable_states_with_preambles M. \<Union> (prefix_pair_tests q ` {m_traversal_paths_with_witness M q RepSets m}))"
                      and   "(\<lambda>(q, p, q'). (q, p)) qzq = (q,z)"
             using scheme[OF 1] by blast
           then obtain q' where "q'\<in>fst ` d_reachable_states_with_preambles M"
-                         and   "qzq \<in> \<Union> (prefix_pair_tests q' ` {m_traversal_paths_with_witness M q' (maximal_repetition_sets_from_separators_list M) m})"
+                         and   "qzq \<in> \<Union> (prefix_pair_tests q' ` {m_traversal_paths_with_witness M q' RepSets m})"
             by blast
           then have "fst qzq = q'"
             by auto
           then have "q' = q"
             using \<open>(\<lambda>(q, p, q'). (q, p)) qzq = (q,z)\<close>
             by (simp add: prod.case_eq_if) 
-          then have "qzq \<in> \<Union> (prefix_pair_tests q ` {m_traversal_paths_with_witness M q (maximal_repetition_sets_from_separators_list M) m})"
-            using \<open>qzq \<in> \<Union> (prefix_pair_tests q' ` {m_traversal_paths_with_witness M q' (maximal_repetition_sets_from_separators_list M) m})\<close> 
+          then have "qzq \<in> \<Union> (prefix_pair_tests q ` {m_traversal_paths_with_witness M q RepSets m})"
+            using \<open>qzq \<in> \<Union> (prefix_pair_tests q' ` {m_traversal_paths_with_witness M q' RepSets m})\<close> 
             by blast
           then have "(\<lambda>(q, p, q'). (q, p)) qzq \<in> ?S2"
             by auto
@@ -485,14 +486,14 @@ proof -
         
 
 
-    show "tps q = (fst ` m_traversal_paths_with_witness M q (maximal_repetition_sets_from_separators_list M) m) \<union> 
+    show "tps q = (fst ` m_traversal_paths_with_witness M q RepSets m) \<union> 
                   {z. (q, z)
                     \<in> (\<lambda>(q, p, q'). (q, p)) `
-                       ((prefix_pair_tests q (m_traversal_paths_with_witness M q (maximal_repetition_sets_from_separators_list M) m)) \<union>
+                       ((prefix_pair_tests q (m_traversal_paths_with_witness M q RepSets m)) \<union>
                         (\<Union>q\<in>fst ` d_reachable_states_with_preambles M.
-                            \<Union>mrsps\<in>{m_traversal_paths_with_witness M q (maximal_repetition_sets_from_separators_list M) m}.
+                            \<Union>mrsps\<in>{m_traversal_paths_with_witness M q RepSets m}.
                                preamble_prefix_tests q mrsps (fst ` d_reachable_states_with_preambles M)) \<union>
-                        preamble_pair_tests (\<Union>(q, y)\<in>(\<lambda>q. (q, m_traversal_paths_with_witness M q (maximal_repetition_sets_from_separators_list M) m)) ` fst ` d_reachable_states_with_preambles M. (\<lambda>(p, rd, dr). dr) ` y) (fst ` (\<lambda>((q1, q2), A). ((q1, q2), A, Inr q1 :: 'a \<times> 'a + 'a, Inr q2 :: 'a \<times> 'a + 'a)) ` r_distinguishable_state_pairs_with_separators M))}"
+                        preamble_pair_tests (\<Union>(q, y)\<in>(\<lambda>q. (q, m_traversal_paths_with_witness M q RepSets m)) ` fst ` d_reachable_states_with_preambles M. (\<lambda>(p, rd, dr). dr) ` y) (fst ` (\<lambda>((q1, q2), A). ((q1, q2), A, Inr q1 :: 'a \<times> 'a + 'a, Inr q2 :: 'a \<times> 'a + 'a)) ` r_distinguishable_state_pairs_with_separators M))}"
      using * unfolding ** by assumption
 
 
@@ -501,11 +502,11 @@ proof -
     have ***: "rd_targets (q,p) = {z. ((q, p), z)
                    \<in> (\<lambda>(q, p, y). ((q, p), y)) `
                       ((\<Union>q\<in>fst ` d_reachable_states_with_preambles M.
-                           \<Union> (prefix_pair_tests q ` {m_traversal_paths_with_witness M q (maximal_repetition_sets_from_separators_list M) m})) \<union>
+                           \<Union> (prefix_pair_tests q ` {m_traversal_paths_with_witness M q RepSets m})) \<union>
                        (\<Union>q\<in>fst ` d_reachable_states_with_preambles M.
-                           \<Union>mrsps\<in>{m_traversal_paths_with_witness M q (maximal_repetition_sets_from_separators_list M) m}.
+                           \<Union>mrsps\<in>{m_traversal_paths_with_witness M q RepSets m}.
                               preamble_prefix_tests q mrsps (fst ` d_reachable_states_with_preambles M)) \<union>
-                       preamble_pair_tests (\<Union>(q, y)\<in>(\<lambda>q. (q, m_traversal_paths_with_witness M q (maximal_repetition_sets_from_separators_list M) m)) ` fst ` d_reachable_states_with_preambles M. (\<lambda>(p, rd, dr). dr) ` y) (fst ` (\<lambda>((q1, q2), A). ((q1, q2), A, Inr q1 :: 'a \<times> 'a + 'a, Inr q2 :: 'a \<times> 'a + 'a)) ` r_distinguishable_state_pairs_with_separators M))}"
+                       preamble_pair_tests (\<Union>(q, y)\<in>(\<lambda>q. (q, m_traversal_paths_with_witness M q RepSets m)) ` fst ` d_reachable_states_with_preambles M. (\<lambda>(p, rd, dr). dr) ` y) (fst ` (\<lambda>((q1, q2), A). ((q1, q2), A, Inr q1 :: 'a \<times> 'a + 'a, Inr q2 :: 'a \<times> 'a + 'a)) ` r_distinguishable_state_pairs_with_separators M))}"
       unfolding rd_targets_def
       unfolding scheme1 scheme2 scheme3 scheme4
       unfolding set_as_map_def
@@ -515,47 +516,47 @@ proof -
     have ****: "{z. ((q, p), z)
                    \<in> (\<lambda>(q, p, y). ((q, p), y)) `
                       ((\<Union>q\<in>fst ` d_reachable_states_with_preambles M.
-                           \<Union> (prefix_pair_tests q ` {m_traversal_paths_with_witness M q (maximal_repetition_sets_from_separators_list M) m})) \<union>
+                           \<Union> (prefix_pair_tests q ` {m_traversal_paths_with_witness M q RepSets m})) \<union>
                        (\<Union>q\<in>fst ` d_reachable_states_with_preambles M.
-                           \<Union>mrsps\<in>{m_traversal_paths_with_witness M q (maximal_repetition_sets_from_separators_list M) m}.
+                           \<Union>mrsps\<in>{m_traversal_paths_with_witness M q RepSets m}.
                               preamble_prefix_tests q mrsps (fst ` d_reachable_states_with_preambles M)) \<union>
-                       preamble_pair_tests (\<Union>(q, y)\<in>(\<lambda>q. (q, m_traversal_paths_with_witness M q (maximal_repetition_sets_from_separators_list M) m)) ` fst ` d_reachable_states_with_preambles M. (\<lambda>(p, rd, dr). dr) ` y) (fst ` (\<lambda>((q1, q2), A). ((q1, q2), A, Inr q1 :: 'a \<times> 'a + 'a, Inr q2 :: 'a \<times> 'a + 'a)) ` r_distinguishable_state_pairs_with_separators M))}
+                       preamble_pair_tests (\<Union>(q, y)\<in>(\<lambda>q. (q, m_traversal_paths_with_witness M q RepSets m)) ` fst ` d_reachable_states_with_preambles M. (\<lambda>(p, rd, dr). dr) ` y) (fst ` (\<lambda>((q1, q2), A). ((q1, q2), A, Inr q1 :: 'a \<times> 'a + 'a, Inr q2 :: 'a \<times> 'a + 'a)) ` r_distinguishable_state_pairs_with_separators M))}
           = {z. ((q, p), z)
                    \<in> (\<lambda>(q, p, y). ((q, p), y)) `
-                      ((prefix_pair_tests q (m_traversal_paths_with_witness M q (maximal_repetition_sets_from_separators_list M) m)) \<union>
+                      ((prefix_pair_tests q (m_traversal_paths_with_witness M q RepSets m)) \<union>
                        (\<Union>q\<in>fst ` d_reachable_states_with_preambles M.
-                           \<Union>mrsps\<in>{m_traversal_paths_with_witness M q (maximal_repetition_sets_from_separators_list M) m}.
+                           \<Union>mrsps\<in>{m_traversal_paths_with_witness M q RepSets m}.
                               preamble_prefix_tests q mrsps (fst ` d_reachable_states_with_preambles M)) \<union>
-                       preamble_pair_tests (\<Union>(q, y)\<in>(\<lambda>q. (q, m_traversal_paths_with_witness M q (maximal_repetition_sets_from_separators_list M) m)) ` fst ` d_reachable_states_with_preambles M. (\<lambda>(p, rd, dr). dr) ` y) (fst ` (\<lambda>((q1, q2), A). ((q1, q2), A, Inr q1 :: 'a \<times> 'a + 'a, Inr q2 :: 'a \<times> 'a + 'a)) ` r_distinguishable_state_pairs_with_separators M))}" 
+                       preamble_pair_tests (\<Union>(q, y)\<in>(\<lambda>q. (q, m_traversal_paths_with_witness M q RepSets m)) ` fst ` d_reachable_states_with_preambles M. (\<lambda>(p, rd, dr). dr) ` y) (fst ` (\<lambda>((q1, q2), A). ((q1, q2), A, Inr q1 :: 'a \<times> 'a + 'a, Inr q2 :: 'a \<times> 'a + 'a)) ` r_distinguishable_state_pairs_with_separators M))}" 
       (is "{z. ((q, p), z) \<in> ?S1} = {z. ((q, p), z) \<in> ?S2}")
     proof -
       have "\<And> z . ((q, p), z) \<in> ?S1 \<Longrightarrow> ((q, p), z) \<in> ?S2"
       proof -
         fix z assume "((q, p), z) \<in> ?S1"
         then consider "((q, p), z) \<in> (\<lambda>(q, p, y). ((q, p), y)) ` (\<Union>q\<in>fst ` d_reachable_states_with_preambles M.
-                            \<Union> (prefix_pair_tests q ` {m_traversal_paths_with_witness M q (maximal_repetition_sets_from_separators_list M) m}))"
+                            \<Union> (prefix_pair_tests q ` {m_traversal_paths_with_witness M q RepSets m}))"
                     | "((q, p), z) \<in> (\<lambda>(q, p, y). ((q, p), y)) `  (\<Union>q\<in>fst ` d_reachable_states_with_preambles M.
-                            \<Union>mrsps\<in>{m_traversal_paths_with_witness M q (maximal_repetition_sets_from_separators_list M) m}.
+                            \<Union>mrsps\<in>{m_traversal_paths_with_witness M q RepSets m}.
                                preamble_prefix_tests q mrsps (fst ` d_reachable_states_with_preambles M))"
-                    | "((q, p), z) \<in> (\<lambda>(q, p, y). ((q, p), y)) ` (preamble_pair_tests (\<Union>(q, y)\<in>(\<lambda>q. (q, m_traversal_paths_with_witness M q (maximal_repetition_sets_from_separators_list M) m)) ` fst ` d_reachable_states_with_preambles M. (\<lambda>(p, rd, dr). dr) ` y) (fst ` (\<lambda>((q1, q2), A). ((q1, q2), A, Inr q1 :: 'a \<times> 'a + 'a, Inr q2 :: 'a \<times> 'a + 'a)) ` r_distinguishable_state_pairs_with_separators M))"
+                    | "((q, p), z) \<in> (\<lambda>(q, p, y). ((q, p), y)) ` (preamble_pair_tests (\<Union>(q, y)\<in>(\<lambda>q. (q, m_traversal_paths_with_witness M q RepSets m)) ` fst ` d_reachable_states_with_preambles M. (\<lambda>(p, rd, dr). dr) ` y) (fst ` (\<lambda>((q1, q2), A). ((q1, q2), A, Inr q1 :: 'a \<times> 'a + 'a, Inr q2 :: 'a \<times> 'a + 'a)) ` r_distinguishable_state_pairs_with_separators M))"
           by blast
         then show "((q, p), z) \<in> ?S2" proof cases
           case 1
           have scheme: "\<And> f y xs . y \<in> image f xs \<Longrightarrow> \<exists> x . x \<in> xs \<and> f x = y" by auto
 
-          obtain qzq where "qzq \<in> (\<Union>q\<in>fst ` d_reachable_states_with_preambles M. \<Union> (prefix_pair_tests q ` {m_traversal_paths_with_witness M q (maximal_repetition_sets_from_separators_list M) m}))"
+          obtain qzq where "qzq \<in> (\<Union>q\<in>fst ` d_reachable_states_with_preambles M. \<Union> (prefix_pair_tests q ` {m_traversal_paths_with_witness M q RepSets m}))"
                      and   "(\<lambda>(q, p, y). ((q, p), y)) qzq = ((q,p),z)"
             using scheme[OF 1] by blast
           then obtain q' where "q'\<in>fst ` d_reachable_states_with_preambles M"
-                         and   "qzq \<in> \<Union> (prefix_pair_tests q' ` {m_traversal_paths_with_witness M q' (maximal_repetition_sets_from_separators_list M) m})"
+                         and   "qzq \<in> \<Union> (prefix_pair_tests q' ` {m_traversal_paths_with_witness M q' RepSets m})"
             by blast
           then have "fst qzq = q'"
             by auto
           then have "q' = q"
             using \<open>(\<lambda>(q, p, y). ((q, p), y)) qzq = ((q,p),z)\<close>
             by (simp add: prod.case_eq_if) 
-          then have "qzq \<in> \<Union> (prefix_pair_tests q ` {m_traversal_paths_with_witness M q (maximal_repetition_sets_from_separators_list M) m})"
-            using \<open>qzq \<in> \<Union> (prefix_pair_tests q' ` {m_traversal_paths_with_witness M q' (maximal_repetition_sets_from_separators_list M) m})\<close> 
+          then have "qzq \<in> \<Union> (prefix_pair_tests q ` {m_traversal_paths_with_witness M q RepSets m})"
+            using \<open>qzq \<in> \<Union> (prefix_pair_tests q' ` {m_traversal_paths_with_witness M q' RepSets m})\<close> 
             by blast
           then have "(\<lambda>(q, p, y). ((q, p), y)) qzq \<in> ?S2"
             by auto
@@ -581,11 +582,11 @@ proof -
 
     show "rd_targets (q,p) = {z. ((q, p), z)
                    \<in> (\<lambda>(q, p, y). ((q, p), y)) `
-                      ((prefix_pair_tests q (m_traversal_paths_with_witness M q (maximal_repetition_sets_from_separators_list M) m)) \<union>
+                      ((prefix_pair_tests q (m_traversal_paths_with_witness M q RepSets m)) \<union>
                        (\<Union>q\<in>fst ` d_reachable_states_with_preambles M.
-                           \<Union>mrsps\<in>{m_traversal_paths_with_witness M q (maximal_repetition_sets_from_separators_list M) m}.
+                           \<Union>mrsps\<in>{m_traversal_paths_with_witness M q RepSets m}.
                               preamble_prefix_tests q mrsps (fst ` d_reachable_states_with_preambles M)) \<union>
-                       preamble_pair_tests (\<Union>(q, y)\<in>(\<lambda>q. (q, m_traversal_paths_with_witness M q (maximal_repetition_sets_from_separators_list M) m)) ` fst ` d_reachable_states_with_preambles M. (\<lambda>(p, rd, dr). dr) ` y) (fst ` (\<lambda>((q1, q2), A). ((q1, q2), A, Inr q1 :: 'a \<times> 'a + 'a, Inr q2 :: 'a \<times> 'a + 'a)) ` r_distinguishable_state_pairs_with_separators M))}"
+                       preamble_pair_tests (\<Union>(q, y)\<in>(\<lambda>q. (q, m_traversal_paths_with_witness M q RepSets m)) ` fst ` d_reachable_states_with_preambles M. (\<lambda>(p, rd, dr). dr) ` y) (fst ` (\<lambda>((q1, q2), A). ((q1, q2), A, Inr q1 :: 'a \<times> 'a + 'a, Inr q2 :: 'a \<times> 'a + 'a)) ` r_distinguishable_state_pairs_with_separators M))}"
       using ***  unfolding **** by assumption
   qed
 
@@ -593,31 +594,31 @@ proof -
 
 
 
-  define pps_alt :: "('a,'b,'c) test_path set" where pps_alt_def : "pps_alt = {(q1,[],q2) | q1 q2 . \<exists> q p rd dr . q \<in> fst ` d_reachable_states_with_preambles M \<and> (p,(rd,dr)) \<in> m_traversal_paths_with_witness M q (maximal_repetition_sets_from_separators_list M) m \<and> q1 \<in> dr \<and> q2 \<in> dr \<and> (q1,q2) \<in> fst  ` r_distinguishable_state_pairs_with_separators M}"
+  define pps_alt :: "('a,'b,'c) test_path set" where pps_alt_def : "pps_alt = {(q1,[],q2) | q1 q2 . \<exists> q p rd dr . q \<in> fst ` d_reachable_states_with_preambles M \<and> (p,(rd,dr)) \<in> m_traversal_paths_with_witness M q RepSets m \<and> q1 \<in> dr \<and> q2 \<in> dr \<and> (q1,q2) \<in> fst  ` r_distinguishable_state_pairs_with_separators M}"
   have preamble_pair_tests_alt :
-    "preamble_pair_tests (\<Union>(q, y)\<in>(\<lambda>q. (q, m_traversal_paths_with_witness M q (maximal_repetition_sets_from_separators_list M) m)) ` fst ` d_reachable_states_with_preambles M. (\<lambda>(p, rd, dr). dr) ` y) (fst ` (\<lambda>((q1, q2), A). ((q1, q2), A, Inr q1 :: 'a \<times> 'a + 'a, Inr q2 :: 'a \<times> 'a + 'a)) ` r_distinguishable_state_pairs_with_separators M)
+    "preamble_pair_tests (\<Union>(q, y)\<in>(\<lambda>q. (q, m_traversal_paths_with_witness M q RepSets m)) ` fst ` d_reachable_states_with_preambles M. (\<lambda>(p, rd, dr). dr) ` y) (fst ` (\<lambda>((q1, q2), A). ((q1, q2), A, Inr q1 :: 'a \<times> 'a + 'a, Inr q2 :: 'a \<times> 'a + 'a)) ` r_distinguishable_state_pairs_with_separators M)
      = pps_alt"
     (is "?PP1 = ?PP2")
   proof -
     have "\<And> x . x \<in> ?PP1 \<Longrightarrow> x \<in> ?PP2"
     proof -
       fix x assume "x \<in> ?PP1"
-      then obtain drs where "drs \<in> (\<Union>(q, y)\<in>(\<lambda>q. (q, m_traversal_paths_with_witness M q (maximal_repetition_sets_from_separators_list M) m)) ` fst ` d_reachable_states_with_preambles M. (\<lambda>(p, rd, dr). dr) ` y)"
+      then obtain drs where "drs \<in> (\<Union>(q, y)\<in>(\<lambda>q. (q, m_traversal_paths_with_witness M q RepSets m)) ` fst ` d_reachable_states_with_preambles M. (\<lambda>(p, rd, dr). dr) ` y)"
                       and   "x \<in> (\<lambda>(q1, q2). (q1, [], q2)) ` (drs \<times> drs \<inter> fst ` (\<lambda>((q1, q2), A). ((q1, q2), A, Inr q1, Inr q2)) ` r_distinguishable_state_pairs_with_separators M)"
         unfolding preamble_pair_tests.simps by force
 
-      obtain q y where "(q,y) \<in> (\<lambda>q. (q, m_traversal_paths_with_witness M q (maximal_repetition_sets_from_separators_list M) m)) ` fst ` d_reachable_states_with_preambles M"
+      obtain q y where "(q,y) \<in> (\<lambda>q. (q, m_traversal_paths_with_witness M q RepSets m)) ` fst ` d_reachable_states_with_preambles M"
                  and   "drs \<in> (\<lambda>(p, rd, dr). dr) ` y"
-        using \<open>drs \<in> (\<Union>(q, y)\<in>(\<lambda>q. (q, m_traversal_paths_with_witness M q (maximal_repetition_sets_from_separators_list M) m)) ` fst ` d_reachable_states_with_preambles M. (\<lambda>(p, rd, dr). dr) ` y)\<close>
+        using \<open>drs \<in> (\<Union>(q, y)\<in>(\<lambda>q. (q, m_traversal_paths_with_witness M q RepSets m)) ` fst ` d_reachable_states_with_preambles M. (\<lambda>(p, rd, dr). dr) ` y)\<close>
         by force
 
       have "q \<in> fst ` d_reachable_states_with_preambles M"
-      and  "y = m_traversal_paths_with_witness M q (maximal_repetition_sets_from_separators_list M) m"
-        using \<open>(q,y) \<in> (\<lambda>q. (q, m_traversal_paths_with_witness M q (maximal_repetition_sets_from_separators_list M) m)) ` fst ` d_reachable_states_with_preambles M\<close>
+      and  "y = m_traversal_paths_with_witness M q RepSets m"
+        using \<open>(q,y) \<in> (\<lambda>q. (q, m_traversal_paths_with_witness M q RepSets m)) ` fst ` d_reachable_states_with_preambles M\<close>
         by force+
 
-      obtain p rd where "(p,(rd,drs)) \<in> m_traversal_paths_with_witness M q (maximal_repetition_sets_from_separators_list M) m"
-        using \<open>drs \<in> (\<lambda>(p, rd, dr). dr) ` y\<close> unfolding \<open>y = m_traversal_paths_with_witness M q (maximal_repetition_sets_from_separators_list M) m\<close>
+      obtain p rd where "(p,(rd,drs)) \<in> m_traversal_paths_with_witness M q RepSets m"
+        using \<open>drs \<in> (\<lambda>(p, rd, dr). dr) ` y\<close> unfolding \<open>y = m_traversal_paths_with_witness M q RepSets m\<close>
         by force
 
 
@@ -632,7 +633,7 @@ proof -
 
       then show "x \<in> ?PP2"
         unfolding \<open>x = (q1, [], q2)\<close> pps_alt_def
-        using \<open>q \<in> fst ` d_reachable_states_with_preambles M\<close> \<open>(p,(rd,drs)) \<in> m_traversal_paths_with_witness M q (maximal_repetition_sets_from_separators_list M) m\<close>
+        using \<open>q \<in> fst ` d_reachable_states_with_preambles M\<close> \<open>(p,(rd,drs)) \<in> m_traversal_paths_with_witness M q RepSets m\<close>
         by blast
     qed
 
@@ -642,12 +643,12 @@ proof -
       then obtain q1 q2 where "x = (q1,[],q2)" unfolding pps_alt_def
         by auto
       then obtain q p rd dr where "q \<in> fst ` d_reachable_states_with_preambles M" 
-                            and   "(p,(rd,dr)) \<in> m_traversal_paths_with_witness M q (maximal_repetition_sets_from_separators_list M) m" 
+                            and   "(p,(rd,dr)) \<in> m_traversal_paths_with_witness M q RepSets m" 
                             and   "q1 \<in> dr \<and> q2 \<in> dr \<and> (q1,q2) \<in> fst  ` r_distinguishable_state_pairs_with_separators M"
         using \<open>x \<in> ?PP2\<close> unfolding pps_alt_def by blast
 
-      have "dr \<in> (\<Union>(q, y)\<in>(\<lambda>q. (q, m_traversal_paths_with_witness M q (maximal_repetition_sets_from_separators_list M) m)) ` fst ` d_reachable_states_with_preambles M. (\<lambda>(p, rd, dr). dr) ` y)"
-        using \<open>q \<in> fst ` d_reachable_states_with_preambles M\<close> \<open>(p,(rd,dr)) \<in> m_traversal_paths_with_witness M q (maximal_repetition_sets_from_separators_list M) m\<close> by force
+      have "dr \<in> (\<Union>(q, y)\<in>(\<lambda>q. (q, m_traversal_paths_with_witness M q RepSets m)) ` fst ` d_reachable_states_with_preambles M. (\<lambda>(p, rd, dr). dr) ` y)"
+        using \<open>q \<in> fst ` d_reachable_states_with_preambles M\<close> \<open>(p,(rd,dr)) \<in> m_traversal_paths_with_witness M q RepSets m\<close> by force
 
       moreover have "x \<in> (\<lambda>(q1, q2). (q1, [], q2)) ` (dr \<times> dr \<inter> fst ` (\<lambda>((q1, q2), A). ((q1, q2), A, Inr q1, Inr q2)) ` r_distinguishable_state_pairs_with_separators M)"
         unfolding \<open>x = (q1,[],q2)\<close> using \<open>q1 \<in> dr \<and> q2 \<in> dr \<and> (q1,q2) \<in> fst  ` r_distinguishable_state_pairs_with_separators M\<close> by force
@@ -676,13 +677,6 @@ proof -
     using assms(1) d_reachable_states_with_preambles_soundness(1) nodes_with_preambles_def by blast
 
 
-  have "\<And>q. q \<in> FSM.nodes M \<Longrightarrow> \<exists>d\<in>set (maximal_repetition_sets_from_separators_list M). q \<in> fst d"
-  and  "\<And>d. d \<in> set (maximal_repetition_sets_from_separators_list M) \<Longrightarrow> snd d \<subseteq> fst d"
-    unfolding maximal_repetition_sets_from_separators_code_alt[symmetric]
-              maximal_repetition_sets_from_separators_def
-    using maximal_pairwise_r_distinguishable_state_sets_from_separators_cover[of _ M] by force+
-
-
   have p2b: "\<And> q P . (q,P) \<in> nodes_with_preambles \<Longrightarrow> (tps q) \<noteq> {}"
   proof -
     fix q P assume "(q,P) \<in> nodes_with_preambles"
@@ -694,19 +688,19 @@ proof -
       using \<open>(q, P) \<in> nodes_with_preambles\<close> assms(1) d_reachable_states_with_preambles_soundness(2) nodes_with_preambles_def by blast 
 
 
-    obtain p' d' where  "(p', d') \<in> m_traversal_paths_with_witness M q (maximal_repetition_sets_from_separators_list M) m"
-      using m_traversal_path_exist[OF assms(2) \<open>q \<in> nodes M\<close> assms(3) \<open>\<And>q. q \<in> FSM.nodes M \<Longrightarrow> \<exists>d\<in>set (maximal_repetition_sets_from_separators_list M). q \<in> fst d\<close> \<open>\<And>d. d \<in> set (maximal_repetition_sets_from_separators_list M) \<Longrightarrow> snd d \<subseteq> fst d\<close>]
+    obtain p' d' where  "(p', d') \<in> m_traversal_paths_with_witness M q RepSets m"
+      using m_traversal_path_exist[OF assms(2) \<open>q \<in> nodes M\<close> assms(3) \<open>\<And>q. q \<in> FSM.nodes M \<Longrightarrow> \<exists>d\<in>set RepSets. q \<in> fst d\<close>] assms(5) 
       by blast
-    then have "p' \<in> image fst (m_traversal_paths_with_witness M q (maximal_repetition_sets_from_separators_list M) m)"
+    then have "p' \<in> image fst (m_traversal_paths_with_witness M q RepSets m)"
       using image_iff by fastforce
     
-    have "(q, image fst (m_traversal_paths_with_witness M q (maximal_repetition_sets_from_separators_list M) m)) \<in> (image (\<lambda> (q,p) . (q, image fst p)) (image (\<lambda> q . (q,m_traversal_paths_with_witness M q (maximal_repetition_sets_from_separators_list M) m)) (image fst (d_reachable_states_with_preambles M))))"
+    have "(q, image fst (m_traversal_paths_with_witness M q RepSets m)) \<in> (image (\<lambda> (q,p) . (q, image fst p)) (image (\<lambda> q . (q,m_traversal_paths_with_witness M q RepSets m)) (image fst (d_reachable_states_with_preambles M))))"
       using \<open>q \<in> (image fst (d_reachable_states_with_preambles M))\<close> by force
-    have "(image fst (m_traversal_paths_with_witness M q (maximal_repetition_sets_from_separators_list M) m)) \<in> (m2f (set_as_map (image (\<lambda> (q,p) . (q, image fst p)) (image (\<lambda> q . (q,m_traversal_paths_with_witness M q (maximal_repetition_sets_from_separators_list M) m)) (image fst (d_reachable_states_with_preambles M)))))) q"
-      using set_as_map_containment[OF \<open>(q, image fst (m_traversal_paths_with_witness M q (maximal_repetition_sets_from_separators_list M) m)) \<in> (image (\<lambda> (q,p) . (q, image fst p)) (image (\<lambda> q . (q,m_traversal_paths_with_witness M q (maximal_repetition_sets_from_separators_list M) m)) (image fst (d_reachable_states_with_preambles M))))\<close>]
+    have "(image fst (m_traversal_paths_with_witness M q RepSets m)) \<in> (m2f (set_as_map (image (\<lambda> (q,p) . (q, image fst p)) (image (\<lambda> q . (q,m_traversal_paths_with_witness M q RepSets m)) (image fst (d_reachable_states_with_preambles M)))))) q"
+      using set_as_map_containment[OF \<open>(q, image fst (m_traversal_paths_with_witness M q RepSets m)) \<in> (image (\<lambda> (q,p) . (q, image fst p)) (image (\<lambda> q . (q,m_traversal_paths_with_witness M q RepSets m)) (image fst (d_reachable_states_with_preambles M))))\<close>]
       by assumption
-    then have "p' \<in> (\<Union> ((m2f (set_as_map (image (\<lambda> (q,p) . (q, image fst p)) (image (\<lambda> q . (q,m_traversal_paths_with_witness M q (maximal_repetition_sets_from_separators_list M) m)) (image fst (d_reachable_states_with_preambles M)))))) q))"
-      using \<open>p' \<in> image fst (m_traversal_paths_with_witness M q (maximal_repetition_sets_from_separators_list M) m)\<close> by blast
+    then have "p' \<in> (\<Union> ((m2f (set_as_map (image (\<lambda> (q,p) . (q, image fst p)) (image (\<lambda> q . (q,m_traversal_paths_with_witness M q RepSets m)) (image fst (d_reachable_states_with_preambles M)))))) q))"
+      using \<open>p' \<in> image fst (m_traversal_paths_with_witness M q RepSets m)\<close> by blast
 
     then show "(tps q) \<noteq> {}"
       unfolding tps_def m2f_by_from_m2f by blast
@@ -751,48 +745,22 @@ proof -
 
 
 
-  let ?RepSets = "(maximal_repetition_sets_from_separators_list M)"
+  let ?RepSets = "RepSets"
 
   have p4: "\<And> q . q \<in> nodes M \<Longrightarrow> (\<exists>d \<in> set ?RepSets. q \<in> fst d)"
-  proof -
-    fix q assume "q \<in> nodes M"
-
-    have *: "image fst (set ?RepSets) = set (maximal_pairwise_r_distinguishable_state_sets_from_separators_list M)"
-      unfolding maximal_repetition_sets_from_separators_list_def
-      by force
-    have "(\<exists>d \<in> image fst (set ?RepSets). q \<in> d)"
-      unfolding * maximal_pairwise_r_distinguishable_state_sets_from_separators_code[symmetric]
-      using maximal_pairwise_r_distinguishable_state_sets_from_separators_cover[OF \<open>q \<in> nodes M\<close>]
-      by assumption
-    then show "(\<exists>d \<in> set ?RepSets. q \<in> fst d)"
-      by auto
-  qed
+    by (simp add: assms(4))
+  
 
       
   have p5: "\<And> d . d \<in> set ?RepSets \<Longrightarrow> ((fst d \<subseteq> nodes M) \<and> (snd d = fst d \<inter> fst ` nodes_with_preambles) \<and> (\<forall> q1 q2 . q1 \<in> fst d \<longrightarrow> q2 \<in> fst d \<longrightarrow> q1 \<noteq> q2 \<longrightarrow> atcs (q1,q2) \<noteq> {}))"
   proof -
     fix d assume "d \<in> set ?RepSets"
-    then have "d \<in> maximal_repetition_sets_from_separators M"
-      unfolding maximal_repetition_sets_from_separators_code_alt[symmetric] 
-      by assumption
     
-
-
-    have "fst d \<subseteq> nodes M" and "(snd d = fst d \<inter> fst ` nodes_with_preambles)" and "\<And> q1 q2 . q1\<in>fst d \<Longrightarrow> q2\<in>fst d \<Longrightarrow> q1 \<noteq> q2 \<Longrightarrow> (q1, q2) \<in> fst ` r_distinguishable_state_pairs_with_separators M"
-      using \<open>d \<in> maximal_repetition_sets_from_separators M\<close>
-      unfolding maximal_repetition_sets_from_separators_def 
-                maximal_pairwise_r_distinguishable_state_sets_from_separators_def
-                pairwise_r_distinguishable_state_sets_from_separators_def 
-                nodes_with_preambles_def
-      by force+
-
-
-    moreover have "\<And> q1 q2 . q1 \<in> fst d \<Longrightarrow> q2 \<in> fst d \<Longrightarrow> q1 \<noteq> q2 \<Longrightarrow> atcs (q1,q2) \<noteq> {}"
+    then have "\<And> q1 q2 . q1 \<in> fst d \<Longrightarrow> q2 \<in> fst d \<Longrightarrow> q1 \<noteq> q2 \<Longrightarrow> atcs (q1,q2) \<noteq> {}"
     proof -
       fix q1 q2 assume "q1 \<in> fst d" and "q2 \<in> fst d" and "q1 \<noteq> q2"
-      then have "(q1, q2) \<in> fst ` r_distinguishable_state_pairs_with_separators M"
-        using \<open>\<And> q1 q2 . q1\<in>fst d \<Longrightarrow> q2\<in>fst d \<Longrightarrow> q1 \<noteq> q2 \<Longrightarrow> (q1, q2) \<in> fst ` r_distinguishable_state_pairs_with_separators M\<close>
-        by blast
+      then have "(q1, q2) \<in> fst ` r_distinguishable_state_pairs_with_separators M" 
+        using assms(6)[OF \<open>d \<in> set ?RepSets\<close>] by blast
       then obtain A where "((q1,q2),A) \<in> r_distinguishable_state_pairs_with_separators M"
         by auto
       then have "(A,Inr q1,Inr q2) \<in> atcs (q1,q2)"
@@ -801,50 +769,51 @@ proof -
       then show "atcs (q1,q2) \<noteq> {}"
         by blast
     qed
-    ultimately show "((fst d \<subseteq> nodes M) \<and> (snd d = fst d \<inter> fst ` nodes_with_preambles) \<and> (\<forall> q1 q2 . q1 \<in> fst d \<longrightarrow> q2 \<in> fst d \<longrightarrow> q1 \<noteq> q2 \<longrightarrow> atcs (q1,q2) \<noteq> {}))"
-      by blast
+    then show "((fst d \<subseteq> nodes M) \<and> (snd d = fst d \<inter> fst ` nodes_with_preambles) \<and> (\<forall> q1 q2 . q1 \<in> fst d \<longrightarrow> q2 \<in> fst d \<longrightarrow> q1 \<noteq> q2 \<longrightarrow> atcs (q1,q2) \<noteq> {}))"
+      using assms(5)[OF \<open>d \<in> set ?RepSets\<close>] unfolding nodes_with_preambles_def by blast
   qed
 
 
 
 
-  have p6 : "\<And> q . q \<in> image fst nodes_with_preambles \<Longrightarrow> tps q \<subseteq> {p1 . \<exists> p2 d . (p1@p2,d) \<in> m_traversal_paths_with_witness M q (maximal_repetition_sets_from_separators_list M) m} \<and> fst ` (m_traversal_paths_with_witness M q (maximal_repetition_sets_from_separators_list M) m) \<subseteq> tps q"
+  have p6 : "\<And> q . q \<in> image fst nodes_with_preambles \<Longrightarrow> tps q \<subseteq> {p1 . \<exists> p2 d . (p1@p2,d) \<in> m_traversal_paths_with_witness M q RepSets m} \<and> fst ` (m_traversal_paths_with_witness M q RepSets m) \<subseteq> tps q"
   proof 
     fix q assume "q \<in> image fst nodes_with_preambles"
     then have "q \<in> fst ` d_reachable_states_with_preambles M"
       unfolding nodes_with_preambles_def by assumption
     then have "q \<in> nodes M"
       by (metis (no_types, lifting) assms(1) d_reachable_states_with_preambles_soundness(2) image_iff prod.collapse)
-    show "fst ` m_traversal_paths_with_witness M q (maximal_repetition_sets_from_separators_list M) m \<subseteq> tps q"
+    show "fst ` m_traversal_paths_with_witness M q RepSets m \<subseteq> tps q"
       unfolding tps_alt_def[OF \<open>q \<in> fst ` d_reachable_states_with_preambles M\<close>]
       by blast
 
-    show "tps q \<subseteq> {p1 . \<exists> p2 d . (p1@p2,d) \<in> m_traversal_paths_with_witness M q (maximal_repetition_sets_from_separators_list M) m}"
+
+    show "tps q \<subseteq> {p1 . \<exists> p2 d . (p1@p2,d) \<in> m_traversal_paths_with_witness M q RepSets m}"
     proof
       fix p assume "p \<in> tps q"
 
 
-      have * : "(\<And> q . q \<in> nodes M \<Longrightarrow> (\<exists>d \<in> set (maximal_repetition_sets_from_separators_list M). q \<in> fst d))" 
+      have * : "(\<And> q . q \<in> nodes M \<Longrightarrow> (\<exists>d \<in> set RepSets. q \<in> fst d))" 
         using p4 by blast
 
-      have  **: "(\<And> d . d \<in> set (maximal_repetition_sets_from_separators_list M) \<Longrightarrow> (snd d \<subseteq> fst d))"
+      have  **: "(\<And> d . d \<in> set RepSets \<Longrightarrow> (snd d \<subseteq> fst d))"
         using p5 by simp
 
       from \<open>p \<in> tps q\<close> consider 
-        (a) "p \<in> fst ` m_traversal_paths_with_witness M q (maximal_repetition_sets_from_separators_list M) m" |
-        (b) "(q, p) \<in> (\<lambda>(q, p, q'). (q, p)) ` (prefix_pair_tests q (m_traversal_paths_with_witness M q (maximal_repetition_sets_from_separators_list M) m))" |
+        (a) "p \<in> fst ` m_traversal_paths_with_witness M q RepSets m" |
+        (b) "(q, p) \<in> (\<lambda>(q, p, q'). (q, p)) ` (prefix_pair_tests q (m_traversal_paths_with_witness M q RepSets m))" |
         (c) "(q, p) \<in> (\<lambda>(q, p, q'). (q, p)) ` (\<Union>q\<in>fst ` d_reachable_states_with_preambles M.
-                \<Union>mrsps\<in>{m_traversal_paths_with_witness M q (maximal_repetition_sets_from_separators_list M) m}.
+                \<Union>mrsps\<in>{m_traversal_paths_with_witness M q RepSets m}.
                    preamble_prefix_tests q mrsps (fst ` d_reachable_states_with_preambles M))" |
         (d) "(q, p) \<in> (\<lambda>(q, p, q'). (q, p)) ` pps_alt"  
         unfolding tps_alt_def[OF \<open>q \<in> fst ` d_reachable_states_with_preambles M\<close>] preamble_pair_tests_alt by blast
 
-      then show "p \<in> {p1. \<exists>p2 d. (p1 @ p2, d) \<in> m_traversal_paths_with_witness M q (maximal_repetition_sets_from_separators_list M) m}"
+      then show "p \<in> {p1. \<exists>p2 d. (p1 @ p2, d) \<in> m_traversal_paths_with_witness M q RepSets m}"
       proof cases
         case a
-        then obtain d where "(p,d) \<in> m_traversal_paths_with_witness M q (maximal_repetition_sets_from_separators_list M) m"
+        then obtain d where "(p,d) \<in> m_traversal_paths_with_witness M q RepSets m"
           by auto
-        then have "\<exists>p2 d. (p @ p2, d) \<in> m_traversal_paths_with_witness M q (maximal_repetition_sets_from_separators_list M) m"
+        then have "\<exists>p2 d. (p @ p2, d) \<in> m_traversal_paths_with_witness M q RepSets m"
           by (metis append_eq_append_conv2)
         then show ?thesis 
           by blast
@@ -852,16 +821,16 @@ proof -
         case b
   
         obtain p1 p2  where "(q,p) \<in> ((\<lambda>(q, p, q'). (q, p)) `{(q, p1, target q p2), (q, p2, target q p1)})"
-           and "\<exists>(p, rd, dr)\<in>m_traversal_paths_with_witness M q (maximal_repetition_sets_from_separators_list M) m.
+           and "\<exists>(p, rd, dr)\<in>m_traversal_paths_with_witness M q RepSets m.
               (p1, p2) \<in> set (prefix_pairs p) \<and> target q p1 \<in> rd \<and> target q p2 \<in> rd \<and> target q p1 \<noteq> target q p2"
           using b
           unfolding prefix_pair_tests.simps by blast
   
         
   
-        obtain p' d where "(p', d) \<in> m_traversal_paths_with_witness M q (maximal_repetition_sets_from_separators_list M) m"
+        obtain p' d where "(p', d) \<in> m_traversal_paths_with_witness M q RepSets m"
                     and   "(p1, p2) \<in> set (prefix_pairs p')"
-          using \<open>\<exists>(p, rd, dr)\<in>m_traversal_paths_with_witness M q (maximal_repetition_sets_from_separators_list M) m.
+          using \<open>\<exists>(p, rd, dr)\<in>m_traversal_paths_with_witness M q RepSets m.
               (p1, p2) \<in> set (prefix_pairs p) \<and> target q p1 \<in> rd \<and> target q p2 \<in> rd \<and> target q p1 \<noteq> target q p2\<close>
           by blast
   
@@ -869,27 +838,27 @@ proof -
           using \<open>(p1, p2) \<in> set (prefix_pairs p')\<close> unfolding prefix_pairs_set_alt 
           using \<open>(q,p) \<in> ((\<lambda>(q, p, q'). (q, p)) `{(q, p1, target q p2), (q, p2, target q p1)})\<close> by auto
         then show ?thesis
-          using \<open>(p', d) \<in> m_traversal_paths_with_witness M q (maximal_repetition_sets_from_separators_list M) m\<close>  
+          using \<open>(p', d) \<in> m_traversal_paths_with_witness M q RepSets m\<close>  
           by blast
       next
         case c     
   
         obtain q' where "q' \<in> fst ` d_reachable_states_with_preambles M"
-                  and   "(q,p) \<in> (\<lambda>(q, p, q'). (q, p)) ` (preamble_prefix_tests q' (m_traversal_paths_with_witness M q' (maximal_repetition_sets_from_separators_list M) m) (fst ` d_reachable_states_with_preambles M))"
+                  and   "(q,p) \<in> (\<lambda>(q, p, q'). (q, p)) ` (preamble_prefix_tests q' (m_traversal_paths_with_witness M q' RepSets m) (fst ` d_reachable_states_with_preambles M))"
           using c by blast
   
         obtain p1 q2  where "(q,p) \<in> ((\<lambda>(q, p, q'). (q, p)) `{(q', p1, q2), (q2, [], target q' p1)})"
-           and "\<exists>(p, rd, dr)\<in>m_traversal_paths_with_witness M q' (maximal_repetition_sets_from_separators_list M) m.
+           and "\<exists>(p, rd, dr)\<in>m_traversal_paths_with_witness M q' RepSets m.
               q2 \<in> fst ` d_reachable_states_with_preambles M \<and> (\<exists>p2. p = p1 @ p2) \<and> target q' p1 \<in> rd \<and> q2 \<in> rd \<and> target q' p1 \<noteq> q2"
-          using \<open>(q,p) \<in> (\<lambda>(q, p, q'). (q, p)) ` (preamble_prefix_tests q' (m_traversal_paths_with_witness M q' (maximal_repetition_sets_from_separators_list M) m) (fst ` d_reachable_states_with_preambles M))\<close>
+          using \<open>(q,p) \<in> (\<lambda>(q, p, q'). (q, p)) ` (preamble_prefix_tests q' (m_traversal_paths_with_witness M q' RepSets m) (fst ` d_reachable_states_with_preambles M))\<close>
           unfolding preamble_prefix_tests_def
           by blast
   
         
   
-        obtain p2 d where "(p1@p2, d)\<in>m_traversal_paths_with_witness M q' (maximal_repetition_sets_from_separators_list M) m"
+        obtain p2 d where "(p1@p2, d)\<in>m_traversal_paths_with_witness M q' RepSets m"
                         and   "q2 \<in> fst ` d_reachable_states_with_preambles M"
-          using \<open>\<exists>(p, rd, dr)\<in>m_traversal_paths_with_witness M q' (maximal_repetition_sets_from_separators_list M) m.
+          using \<open>\<exists>(p, rd, dr)\<in>m_traversal_paths_with_witness M q' RepSets m.
               q2 \<in> fst ` d_reachable_states_with_preambles M \<and> (\<exists>p2. p = p1 @ p2) \<and> target q' p1 \<in> rd \<and> q2 \<in> rd \<and> target q' p1 \<noteq> q2\<close>
           by blast
   
@@ -898,7 +867,7 @@ proof -
         then show ?thesis proof cases
           case a
           then show ?thesis
-            using \<open>(p1 @ p2, d) \<in> m_traversal_paths_with_witness M q' (maximal_repetition_sets_from_separators_list M) m\<close> by blast 
+            using \<open>(p1 @ p2, d) \<in> m_traversal_paths_with_witness M q' RepSets m\<close> by blast 
   
         next
           case b
@@ -906,7 +875,7 @@ proof -
           then have "q \<in> nodes M" and "p = []"
             using \<open>q2 \<in> fst ` d_reachable_states_with_preambles M\<close> unfolding d_reachable_states_with_preambles_def by auto
   
-          have "\<exists>p' d'. (p', d') \<in> m_traversal_paths_with_witness M q (maximal_repetition_sets_from_separators_list M) m"
+          have "\<exists>p' d'. (p', d') \<in> m_traversal_paths_with_witness M q RepSets m"
             using m_traversal_path_exist[OF assms(2) \<open>q \<in> nodes M\<close> assms(3) * **]
             by blast
           then show ?thesis 
@@ -921,7 +890,7 @@ proof -
         have "q \<in> nodes M"
           using \<open>q \<in> fst ` d_reachable_states_with_preambles M\<close> unfolding d_reachable_states_with_preambles_def by auto
   
-        have "\<exists>p' d'. (p', d') \<in> m_traversal_paths_with_witness M q (maximal_repetition_sets_from_separators_list M) m"
+        have "\<exists>p' d'. (p', d') \<in> m_traversal_paths_with_witness M q RepSets m"
           using m_traversal_path_exist[OF assms(2) \<open>q \<in> nodes M\<close> assms(3) * **]
           by blast
         then show ?thesis 
@@ -959,8 +928,8 @@ proof -
             (filter (\<lambda>(p1, p2). target q p1 \<in> fst d \<and> target q p2 \<in> fst d \<and> target q p1 \<noteq> target q p2) (prefix_pairs p)))))"
         using map_set[OF \<open>(p1,p1@p2) \<in> set (filter (\<lambda>(p1, p2). target q p1 \<in> fst d \<and> target q p2 \<in> fst d \<and> target q p1 \<noteq> target q p2) (prefix_pairs p))\<close>, of "(\<lambda>(p1, p2). {(q, p1, target q p2), (q, p2, target q p1)})"] 
         by force
-      then have "(q, p1, target q (p1@p2)) \<in> prefix_pair_tests q (m_traversal_paths_with_witness M q (maximal_repetition_sets_from_separators_list M) m)"
-           and  "(q, p1@p2, target q p1) \<in> prefix_pair_tests q (m_traversal_paths_with_witness M q (maximal_repetition_sets_from_separators_list M) m)"
+      then have "(q, p1, target q (p1@p2)) \<in> prefix_pair_tests q (m_traversal_paths_with_witness M q RepSets m)"
+           and  "(q, p1@p2, target q p1) \<in> prefix_pair_tests q (m_traversal_paths_with_witness M q RepSets m)"
         unfolding prefix_pair_tests_code[of q "m_traversal_paths_with_witness M q ?RepSets m"]
         using \<open>(p,(fst d, snd d)) \<in> m_traversal_paths_with_witness M q ?RepSets m\<close>
         by blast+
@@ -971,8 +940,8 @@ proof -
         
       have "p1 \<in> tps q"
       proof -
-        have "(q, p1) \<in> ((\<lambda>(q, p, q'). (q, p)) ` (prefix_pair_tests q (m_traversal_paths_with_witness M q (maximal_repetition_sets_from_separators_list M) m)))"
-          using \<open>(q, p1, target q (p1@p2)) \<in> prefix_pair_tests q (m_traversal_paths_with_witness M q (maximal_repetition_sets_from_separators_list M) m)\<close>
+        have "(q, p1) \<in> ((\<lambda>(q, p, q'). (q, p)) ` (prefix_pair_tests q (m_traversal_paths_with_witness M q RepSets m)))"
+          using \<open>(q, p1, target q (p1@p2)) \<in> prefix_pair_tests q (m_traversal_paths_with_witness M q RepSets m)\<close>
           by (simp add: rev_image_eqI)  
         then show ?thesis 
           unfolding tps_alt_def[OF \<open>q \<in> fst ` d_reachable_states_with_preambles M\<close>] 
@@ -981,8 +950,8 @@ proof -
 
       moreover have "(p1@p2) \<in> tps q"
       proof -
-        have "(q, p1@p2) \<in> ((\<lambda>(q, p, q'). (q, p)) ` (prefix_pair_tests q (m_traversal_paths_with_witness M q (maximal_repetition_sets_from_separators_list M) m)))"
-          using \<open>(q, p1@p2, target q p1) \<in> prefix_pair_tests q (m_traversal_paths_with_witness M q (maximal_repetition_sets_from_separators_list M) m)\<close>
+        have "(q, p1@p2) \<in> ((\<lambda>(q, p, q'). (q, p)) ` (prefix_pair_tests q (m_traversal_paths_with_witness M q RepSets m)))"
+          using \<open>(q, p1@p2, target q p1) \<in> prefix_pair_tests q (m_traversal_paths_with_witness M q RepSets m)\<close>
           by (simp add: rev_image_eqI) 
         then show ?thesis 
           unfolding tps_alt_def[OF \<open>q \<in> fst ` d_reachable_states_with_preambles M\<close>] 
@@ -991,8 +960,8 @@ proof -
 
       moreover have "target q p1 \<in> rd_targets (q,(p1@p2))"
       proof -
-        have "((q, p1@p2), target q p1) \<in> (\<lambda>(q, p, y). ((q, p), y)) ` prefix_pair_tests q (m_traversal_paths_with_witness M q (maximal_repetition_sets_from_separators_list M) m)"
-          using \<open>(q, p1@p2, target q p1) \<in> prefix_pair_tests q (m_traversal_paths_with_witness M q (maximal_repetition_sets_from_separators_list M) m)\<close>
+        have "((q, p1@p2), target q p1) \<in> (\<lambda>(q, p, y). ((q, p), y)) ` prefix_pair_tests q (m_traversal_paths_with_witness M q RepSets m)"
+          using \<open>(q, p1@p2, target q p1) \<in> prefix_pair_tests q (m_traversal_paths_with_witness M q RepSets m)\<close>
           by (simp add: rev_image_eqI)
         then show ?thesis
           unfolding rd_targets_alt_def[OF \<open>q \<in> fst ` d_reachable_states_with_preambles M\<close>] 
@@ -1001,8 +970,8 @@ proof -
 
       moreover have "target q (p1@p2) \<in> rd_targets (q,p1)"
       proof -
-        have "((q, p1), target q (p1@p2)) \<in> (\<lambda>(q, p, y). ((q, p), y)) ` prefix_pair_tests q (m_traversal_paths_with_witness M q (maximal_repetition_sets_from_separators_list M) m)"
-          using \<open>(q, p1, target q (p1@p2)) \<in> prefix_pair_tests q (m_traversal_paths_with_witness M q (maximal_repetition_sets_from_separators_list M) m)\<close>
+        have "((q, p1), target q (p1@p2)) \<in> (\<lambda>(q, p, y). ((q, p), y)) ` prefix_pair_tests q (m_traversal_paths_with_witness M q RepSets m)"
+          using \<open>(q, p1, target q (p1@p2)) \<in> prefix_pair_tests q (m_traversal_paths_with_witness M q RepSets m)\<close>
           by (simp add: rev_image_eqI)
         then show ?thesis
           unfolding rd_targets_alt_def[OF \<open>q \<in> fst ` d_reachable_states_with_preambles M\<close>] 
@@ -1025,34 +994,34 @@ proof -
       then have "(p1,q') \<in> Set.filter (\<lambda>(p1, q2). target q p1 \<in> fst d \<and> q2 \<in> fst d \<and> target q p1 \<noteq> q2) (set (prefixes p) \<times> fst ` d_reachable_states_with_preambles M)"
         using \<open>target q p1 \<in> fst d\<close> \<open>q' \<in> fst d\<close> \<open>q' \<in> image fst nodes_with_preambles\<close> \<open>target q p1 \<noteq> q'\<close> unfolding nodes_with_preambles_def
         by force
-      then have "{(q, p1, q'), (q', [], target q p1)} \<subseteq> preamble_prefix_tests q (m_traversal_paths_with_witness M q (maximal_repetition_sets_from_separators_list M) m) (fst ` d_reachable_states_with_preambles M)"
+      then have "{(q, p1, q'), (q', [], target q p1)} \<subseteq> preamble_prefix_tests q (m_traversal_paths_with_witness M q RepSets m) (fst ` d_reachable_states_with_preambles M)"
         using preamble_prefix_tests_code[of q "m_traversal_paths_with_witness M q ?RepSets m" "(fst ` d_reachable_states_with_preambles M)"]
         using \<open>(p,(fst d, snd d)) \<in> m_traversal_paths_with_witness M q ?RepSets m\<close>
         by blast
-      then have "(q, p1, q') \<in> preamble_prefix_tests q (m_traversal_paths_with_witness M q (maximal_repetition_sets_from_separators_list M) m) (fst ` d_reachable_states_with_preambles M)"
-           and  "(q', [], target q p1) \<in> preamble_prefix_tests q (m_traversal_paths_with_witness M q (maximal_repetition_sets_from_separators_list M) m) (fst ` d_reachable_states_with_preambles M)"
+      then have "(q, p1, q') \<in> preamble_prefix_tests q (m_traversal_paths_with_witness M q RepSets m) (fst ` d_reachable_states_with_preambles M)"
+           and  "(q', [], target q p1) \<in> preamble_prefix_tests q (m_traversal_paths_with_witness M q RepSets m) (fst ` d_reachable_states_with_preambles M)"
         by blast+
 
       have "p1 \<in> tps q"
-        using \<open>(q, p1, q') \<in> preamble_prefix_tests q (m_traversal_paths_with_witness M q (maximal_repetition_sets_from_separators_list M) m) (fst ` d_reachable_states_with_preambles M)\<close>        
+        using \<open>(q, p1, q') \<in> preamble_prefix_tests q (m_traversal_paths_with_witness M q RepSets m) (fst ` d_reachable_states_with_preambles M)\<close>        
               \<open>q \<in> fst ` d_reachable_states_with_preambles M\<close>
         unfolding tps_alt_def[OF \<open>q \<in> fst ` d_reachable_states_with_preambles M\<close>]
         by force
 
       moreover have "[] \<in> tps q'"
-        using \<open>(q', [], target q p1) \<in> preamble_prefix_tests q (m_traversal_paths_with_witness M q (maximal_repetition_sets_from_separators_list M) m) (fst ` d_reachable_states_with_preambles M)\<close>        
+        using \<open>(q', [], target q p1) \<in> preamble_prefix_tests q (m_traversal_paths_with_witness M q RepSets m) (fst ` d_reachable_states_with_preambles M)\<close>        
               \<open>q \<in> fst ` d_reachable_states_with_preambles M\<close>
         unfolding tps_alt_def[OF \<open>q' \<in> fst ` d_reachable_states_with_preambles M\<close>]
         by force
 
       moreover have "target q p1 \<in> rd_targets (q',[])"
-        using \<open>(q', [], target q p1) \<in> preamble_prefix_tests q (m_traversal_paths_with_witness M q (maximal_repetition_sets_from_separators_list M) m) (fst ` d_reachable_states_with_preambles M)\<close>        
+        using \<open>(q', [], target q p1) \<in> preamble_prefix_tests q (m_traversal_paths_with_witness M q RepSets m) (fst ` d_reachable_states_with_preambles M)\<close>        
               \<open>q \<in> fst ` d_reachable_states_with_preambles M\<close>
         unfolding rd_targets_alt_def[OF \<open>q' \<in> fst ` d_reachable_states_with_preambles M\<close>] 
         by force
 
       moreover have "q' \<in> rd_targets (q,p1)"
-        using \<open>(q, p1, q') \<in> preamble_prefix_tests q (m_traversal_paths_with_witness M q (maximal_repetition_sets_from_separators_list M) m) (fst ` d_reachable_states_with_preambles M)\<close>        
+        using \<open>(q, p1, q') \<in> preamble_prefix_tests q (m_traversal_paths_with_witness M q RepSets m) (fst ` d_reachable_states_with_preambles M)\<close>        
               \<open>q \<in> fst ` d_reachable_states_with_preambles M\<close>
         unfolding rd_targets_alt_def[OF \<open>q \<in> fst ` d_reachable_states_with_preambles M\<close>]
         by force
@@ -1066,19 +1035,19 @@ proof -
     proof -
       fix q1 q2 assume "q1 \<noteq> q2" and "q1 \<in> snd d" and "q2 \<in> snd d"
 
-      have "(\<And>d. d \<in> set (maximal_repetition_sets_from_separators_list M) \<Longrightarrow> snd d \<subseteq> fst d)"
+      have "(\<And>d. d \<in> set RepSets \<Longrightarrow> snd d \<subseteq> fst d)"
         using p5 by blast
       have "q \<in> nodes M"
         by (metis (no_types, lifting) \<open>q \<in> fst ` d_reachable_states_with_preambles M\<close> assms(1) d_reachable_states_with_preambles_soundness(2) image_iff prod.collapse) 
 
-      have "d \<in> set (maximal_repetition_sets_from_separators_list M)" 
-        using m_traversal_paths_with_witness_set[OF p4 \<open>(\<And>d. d \<in> set (maximal_repetition_sets_from_separators_list M) \<Longrightarrow> snd d \<subseteq> fst d)\<close> \<open>q \<in> nodes M\<close>, of m]
-        using \<open>(p, d) \<in> m_traversal_paths_with_witness M q (maximal_repetition_sets_from_separators_list M) m\<close> find_set by force 
+      have "d \<in> set RepSets" 
+        using m_traversal_paths_with_witness_set[OF p4 \<open>(\<And>d. d \<in> set RepSets \<Longrightarrow> snd d \<subseteq> fst d)\<close> \<open>q \<in> nodes M\<close>, of m]
+        using \<open>(p, d) \<in> m_traversal_paths_with_witness M q RepSets m\<close> find_set by force 
 
       have "fst d \<subseteq> nodes M" 
       and  "snd d = fst d \<inter> fst ` nodes_with_preambles" 
       and  "\<And> q1 q2. q1 \<in> fst d \<Longrightarrow> q2 \<in> fst d \<Longrightarrow> q1 \<noteq> q2 \<Longrightarrow> atcs (q1, q2) \<noteq> {}"
-        using p5[OF \<open>d \<in> set (maximal_repetition_sets_from_separators_list M)\<close>] by blast+
+        using p5[OF \<open>d \<in> set RepSets\<close>] by blast+
 
       have "q1 \<in> fst d" and "q2 \<in> fst d" and "q1 \<in> fst ` d_reachable_states_with_preambles M" and "q2 \<in> fst ` d_reachable_states_with_preambles M"
         using \<open>q1 \<in> snd d\<close> \<open>q2 \<in> snd d\<close> unfolding \<open>snd d = fst d \<inter> fst ` nodes_with_preambles\<close> unfolding nodes_with_preambles_def by blast+
@@ -1124,13 +1093,13 @@ proof -
     using p1 p2 p3 p4 p5 p6 p7
     by force
 
-  then show "is_sufficient_for_reduction_testing (calculate_test_suite_example M m) M m"
-    unfolding \<open>calculate_test_suite_example M m = Test_Suite nodes_with_preambles tps rd_targets atcs\<close>
+  then show "is_sufficient_for_reduction_testing (calculate_test_suite_for_repetition_sets M m RepSets) M m"
+    unfolding \<open>calculate_test_suite_for_repetition_sets M m RepSets = Test_Suite nodes_with_preambles tps rd_targets atcs\<close>
               is_sufficient_for_reduction_testing_def
     by blast
 
 
-  show "is_finite_test_suite (calculate_test_suite_example M m)"
+  show "is_finite_test_suite (calculate_test_suite_for_repetition_sets M m RepSets)"
   proof -
     have "finite nodes_with_preambles"
       unfolding nodes_with_preambles_def d_reachable_states_with_preambles_def 
@@ -1143,12 +1112,12 @@ proof -
       fix q p assume "q \<in> fst ` nodes_with_preambles"
       then have "q \<in> fst ` d_reachable_states_with_preambles M" unfolding nodes_with_preambles_def by assumption
 
-      have *: "finite ((\<lambda>(q, p, y). ((q, p), y)) ` (prefix_pair_tests q (m_traversal_paths_with_witness M q (maximal_repetition_sets_from_separators_list M) m) \<union>
+      have *: "finite ((\<lambda>(q, p, y). ((q, p), y)) ` (prefix_pair_tests q (m_traversal_paths_with_witness M q RepSets m) \<union>
              (\<Union>q\<in>fst ` d_reachable_states_with_preambles M.
-                 \<Union>mrsps\<in>{m_traversal_paths_with_witness M q (maximal_repetition_sets_from_separators_list M) m}.
+                 \<Union>mrsps\<in>{m_traversal_paths_with_witness M q RepSets m}.
                     preamble_prefix_tests q mrsps (fst ` d_reachable_states_with_preambles M)) \<union>
              preamble_pair_tests
-              (\<Union>(q, y)\<in>(\<lambda>q. (q, m_traversal_paths_with_witness M q (maximal_repetition_sets_from_separators_list M) m)) `
+              (\<Union>(q, y)\<in>(\<lambda>q. (q, m_traversal_paths_with_witness M q RepSets m)) `
                         fst ` d_reachable_states_with_preambles M.
                   (\<lambda>(p, rd, dr). dr) ` y)
               (fst ` (\<lambda>((q1, q2), A). ((q1, q2), A, Inr q1, Inr q2)) ` r_distinguishable_state_pairs_with_separators M)))"
@@ -1158,15 +1127,15 @@ proof -
 
 
 
-        have "finite ((\<lambda>(q, p, y). ((q, p), y)) ` (prefix_pair_tests q (m_traversal_paths_with_witness M q (maximal_repetition_sets_from_separators_list M) m)))"
+        have "finite ((\<lambda>(q, p, y). ((q, p), y)) ` (prefix_pair_tests q (m_traversal_paths_with_witness M q RepSets m)))"
         proof -
-          have "prefix_pair_tests q (m_traversal_paths_with_witness M q (maximal_repetition_sets_from_separators_list M) m) \<subseteq> 
-                    (\<Union> (p, rd, dr)\<in>m_traversal_paths_with_witness M q (maximal_repetition_sets_from_separators_list M) m . \<Union> (p1, p2) \<in> set (prefix_pairs p) .{(q, p1, target q p2), (q, p2, target q p1)})"
+          have "prefix_pair_tests q (m_traversal_paths_with_witness M q RepSets m) \<subseteq> 
+                    (\<Union> (p, rd, dr)\<in>m_traversal_paths_with_witness M q RepSets m . \<Union> (p1, p2) \<in> set (prefix_pairs p) .{(q, p1, target q p2), (q, p2, target q p1)})"
             unfolding prefix_pair_tests.simps by blast
-          moreover have "finite (\<Union> (p, rd, dr)\<in>m_traversal_paths_with_witness M q (maximal_repetition_sets_from_separators_list M) m . \<Union> (p1, p2) \<in> set (prefix_pairs p) .{(q, p1, target q p2), (q, p2, target q p1)})"
+          moreover have "finite (\<Union> (p, rd, dr)\<in>m_traversal_paths_with_witness M q RepSets m . \<Union> (p1, p2) \<in> set (prefix_pairs p) .{(q, p1, target q p2), (q, p2, target q p1)})"
           proof -
-            have "finite (m_traversal_paths_with_witness M q (maximal_repetition_sets_from_separators_list M) m)"
-              using m_traversal_paths_with_witness_finite[of M q "maximal_repetition_sets_from_separators_list M" m] by assumption
+            have "finite (m_traversal_paths_with_witness M q RepSets m)"
+              using m_traversal_paths_with_witness_finite[of M q "RepSets" m] by assumption
             moreover have "\<And> p rd dr . finite (\<Union> (p1, p2) \<in> set (prefix_pairs p) .{(q, p1, target q p2), (q, p2, target q p1)})"
               by auto
             ultimately show ?thesis by force
@@ -1175,71 +1144,71 @@ proof -
         qed
 
         moreover have "finite ((\<lambda>(q, p, y). ((q, p), y)) ` (\<Union>q\<in>fst ` d_reachable_states_with_preambles M.
-                 \<Union>mrsps\<in>{m_traversal_paths_with_witness M q (maximal_repetition_sets_from_separators_list M) m}.
+                 \<Union>mrsps\<in>{m_traversal_paths_with_witness M q RepSets m}.
                     preamble_prefix_tests q mrsps (fst ` d_reachable_states_with_preambles M)))"
         proof -
           have "finite (fst ` d_reachable_states_with_preambles M)" using \<open>finite nodes_with_preambles\<close> unfolding nodes_with_preambles_def by auto
-          moreover have "\<And> q . q\<in>fst ` d_reachable_states_with_preambles M \<Longrightarrow> finite (\<Union>mrsps\<in>{m_traversal_paths_with_witness M q (maximal_repetition_sets_from_separators_list M) m}. preamble_prefix_tests q mrsps (fst ` d_reachable_states_with_preambles M))"
+          moreover have "\<And> q . q\<in>fst ` d_reachable_states_with_preambles M \<Longrightarrow> finite (\<Union>mrsps\<in>{m_traversal_paths_with_witness M q RepSets m}. preamble_prefix_tests q mrsps (fst ` d_reachable_states_with_preambles M))"
           proof -
             fix q assume "q\<in>fst ` d_reachable_states_with_preambles M"
 
-            have "finite {m_traversal_paths_with_witness M q (maximal_repetition_sets_from_separators_list M) m}" by simp
-            moreover have "\<And> mrsps . mrsps\<in>{m_traversal_paths_with_witness M q (maximal_repetition_sets_from_separators_list M) m} \<Longrightarrow> finite (preamble_prefix_tests q mrsps (fst ` d_reachable_states_with_preambles M))"
+            have "finite {m_traversal_paths_with_witness M q RepSets m}" by simp
+            moreover have "\<And> mrsps . mrsps\<in>{m_traversal_paths_with_witness M q RepSets m} \<Longrightarrow> finite (preamble_prefix_tests q mrsps (fst ` d_reachable_states_with_preambles M))"
             proof -
-              fix mrsps assume "mrsps\<in>{m_traversal_paths_with_witness M q (maximal_repetition_sets_from_separators_list M) m}"
-              then have *: "mrsps = m_traversal_paths_with_witness M q (maximal_repetition_sets_from_separators_list M) m" by simp
+              fix mrsps assume "mrsps\<in>{m_traversal_paths_with_witness M q RepSets m}"
+              then have *: "mrsps = m_traversal_paths_with_witness M q RepSets m" by simp
 
 
               have "preamble_prefix_tests q mrsps (fst ` d_reachable_states_with_preambles M) 
-                      \<subseteq> (\<Union> (p,rd,dr) \<in> m_traversal_paths_with_witness M q (maximal_repetition_sets_from_separators_list M) m . \<Union> q2 \<in> (fst ` d_reachable_states_with_preambles M) . (\<Union> p1 \<in> set (prefixes p) . {(q,p1,q2), (q2,[],(target q p1))}))"              
+                      \<subseteq> (\<Union> (p,rd,dr) \<in> m_traversal_paths_with_witness M q RepSets m . \<Union> q2 \<in> (fst ` d_reachable_states_with_preambles M) . (\<Union> p1 \<in> set (prefixes p) . {(q,p1,q2), (q2,[],(target q p1))}))"              
                 unfolding preamble_prefix_tests_def * prefixes_set by blast
-              moreover have "finite (\<Union> (p,rd,dr) \<in> m_traversal_paths_with_witness M q (maximal_repetition_sets_from_separators_list M) m . \<Union> q2 \<in> (fst ` d_reachable_states_with_preambles M) . (\<Union> p1 \<in> set (prefixes p) . {(q,p1,q2), (q2,[],(target q p1))}))"
+              moreover have "finite (\<Union> (p,rd,dr) \<in> m_traversal_paths_with_witness M q RepSets m . \<Union> q2 \<in> (fst ` d_reachable_states_with_preambles M) . (\<Union> p1 \<in> set (prefixes p) . {(q,p1,q2), (q2,[],(target q p1))}))"
               proof -
-                have "finite (m_traversal_paths_with_witness M q (maximal_repetition_sets_from_separators_list M) m)"
+                have "finite (m_traversal_paths_with_witness M q RepSets m)"
                   using m_traversal_paths_with_witness_finite by metis
-                moreover have "\<And> p rd dr . (p,rd,dr) \<in> m_traversal_paths_with_witness M q (maximal_repetition_sets_from_separators_list M) m \<Longrightarrow> finite (\<Union> q2 \<in> (fst ` d_reachable_states_with_preambles M) . (\<Union> p1 \<in> set (prefixes p) . {(q,p1,q2), (q2,[],(target q p1))}))"
+                moreover have "\<And> p rd dr . (p,rd,dr) \<in> m_traversal_paths_with_witness M q RepSets m \<Longrightarrow> finite (\<Union> q2 \<in> (fst ` d_reachable_states_with_preambles M) . (\<Union> p1 \<in> set (prefixes p) . {(q,p1,q2), (q2,[],(target q p1))}))"
                   using \<open>finite (fst ` d_reachable_states_with_preambles M)\<close> by blast
                 ultimately show ?thesis by force
               qed
               ultimately show "finite (preamble_prefix_tests q mrsps (fst ` d_reachable_states_with_preambles M))" using infinite_super by blast
             qed
-            ultimately show "finite (\<Union>mrsps\<in>{m_traversal_paths_with_witness M q (maximal_repetition_sets_from_separators_list M) m}. preamble_prefix_tests q mrsps (fst ` d_reachable_states_with_preambles M))" by force
+            ultimately show "finite (\<Union>mrsps\<in>{m_traversal_paths_with_witness M q RepSets m}. preamble_prefix_tests q mrsps (fst ` d_reachable_states_with_preambles M))" by force
           qed
           ultimately show ?thesis by blast
         qed
 
         moreover have "finite ((\<lambda>(q, p, y). ((q, p), y)) ` (preamble_pair_tests
-              (\<Union>(q, y)\<in>(\<lambda>q. (q, m_traversal_paths_with_witness M q (maximal_repetition_sets_from_separators_list M) m)) `
+              (\<Union>(q, y)\<in>(\<lambda>q. (q, m_traversal_paths_with_witness M q RepSets m)) `
                         fst ` d_reachable_states_with_preambles M.
                   (\<lambda>(p, rd, dr). dr) ` y)
               (fst ` (\<lambda>((q1, q2), A). ((q1, q2), A, Inr q1, Inr q2)) ` r_distinguishable_state_pairs_with_separators M)))"
         proof -
 
-          have "finite (\<Union>(q, y)\<in>(\<lambda>q. (q, m_traversal_paths_with_witness M q (maximal_repetition_sets_from_separators_list M) m)) `
+          have "finite (\<Union>(q, y)\<in>(\<lambda>q. (q, m_traversal_paths_with_witness M q RepSets m)) `
                         fst ` d_reachable_states_with_preambles M.
                   (\<lambda>(p, rd, dr). dr) ` y)"
           proof -
 
-            have *: "(\<Union>(q, y)\<in>(\<lambda>q. (q, m_traversal_paths_with_witness M q (maximal_repetition_sets_from_separators_list M) m)) `
+            have *: "(\<Union>(q, y)\<in>(\<lambda>q. (q, m_traversal_paths_with_witness M q RepSets m)) `
                         fst ` d_reachable_states_with_preambles M.
                   (\<lambda>(p, rd, dr). dr) ` y) =
-                  (\<Union> q \<in> fst ` d_reachable_states_with_preambles M . \<Union> (p, rd, dr) \<in> m_traversal_paths_with_witness M q (maximal_repetition_sets_from_separators_list M) m . {dr})"
+                  (\<Union> q \<in> fst ` d_reachable_states_with_preambles M . \<Union> (p, rd, dr) \<in> m_traversal_paths_with_witness M q RepSets m . {dr})"
               by force
 
-            have "finite (\<Union> q \<in> fst ` d_reachable_states_with_preambles M . \<Union> (p, rd, dr) \<in> m_traversal_paths_with_witness M q (maximal_repetition_sets_from_separators_list M) m . {dr})"
+            have "finite (\<Union> q \<in> fst ` d_reachable_states_with_preambles M . \<Union> (p, rd, dr) \<in> m_traversal_paths_with_witness M q RepSets m . {dr})"
             proof -
               have "finite (fst ` d_reachable_states_with_preambles M)"
                 using \<open>finite nodes_with_preambles\<close> unfolding nodes_with_preambles_def by auto
 
-              moreover have "\<And>q . q \<in> fst ` d_reachable_states_with_preambles M \<Longrightarrow> finite (\<Union> (p, rd, dr) \<in> m_traversal_paths_with_witness M q (maximal_repetition_sets_from_separators_list M) m . {dr})"
+              moreover have "\<And>q . q \<in> fst ` d_reachable_states_with_preambles M \<Longrightarrow> finite (\<Union> (p, rd, dr) \<in> m_traversal_paths_with_witness M q RepSets m . {dr})"
               proof -
                 fix q assume "q \<in> fst ` d_reachable_states_with_preambles M"
 
-                have "finite (m_traversal_paths_with_witness M q (maximal_repetition_sets_from_separators_list M) m)"
+                have "finite (m_traversal_paths_with_witness M q RepSets m)"
                   using  m_traversal_paths_with_witness_finite by metis 
-                moreover have "\<And> p rd dr . (p, rd, dr) \<in> m_traversal_paths_with_witness M q (maximal_repetition_sets_from_separators_list M) m \<Longrightarrow> finite {dr}"
+                moreover have "\<And> p rd dr . (p, rd, dr) \<in> m_traversal_paths_with_witness M q RepSets m \<Longrightarrow> finite {dr}"
                   by simp
-                ultimately show "finite (\<Union> (p, rd, dr) \<in> m_traversal_paths_with_witness M q (maximal_repetition_sets_from_separators_list M) m . {dr})"
+                ultimately show "finite (\<Union> (p, rd, dr) \<in> m_traversal_paths_with_witness M q RepSets m . {dr})"
                   by force
               qed
               ultimately show ?thesis by blast
@@ -1310,7 +1279,7 @@ proof -
 
 
     ultimately show ?thesis 
-      unfolding \<open>calculate_test_suite_example M m = Test_Suite nodes_with_preambles tps rd_targets atcs\<close>
+      unfolding \<open>calculate_test_suite_for_repetition_sets M m  RepSets = Test_Suite nodes_with_preambles tps rd_targets atcs\<close>
                 is_finite_test_suite.simps 
       by blast
   qed
@@ -1320,9 +1289,20 @@ qed
 
 
 
-subsection \<open>Completeness of the Calculated Test Suite\<close>
 
-lemma calculate_test_suite_example_completeness :
+subsection \<open>Two Complete Example Implementations\<close>
+
+subsubsection \<open>Naive Repetition Set Strategy\<close>
+
+(* Calculates all possible state sets and checks whether they are maximal and pairwise r-distinguishable *)
+definition calculate_test_suite_naive :: "('a::linorder,'b::linorder,'c::linorder) fsm \<Rightarrow> nat \<Rightarrow> ('a,'b,'c, ('a \<times> 'a) + 'a) test_suite" where
+  "calculate_test_suite_naive M m = calculate_test_suite_for_repetition_sets M m (maximal_repetition_sets_from_separators_list_naive M)" 
+
+definition calculate_test_suite_naive_as_io_sequences :: "('a::linorder,'b::linorder,'c::linorder) fsm \<Rightarrow> nat \<Rightarrow> ('b \<times> 'c) list set" where
+  "calculate_test_suite_naive_as_io_sequences M m = test_suite_to_io'_maximal M (calculate_test_suite_naive M m)"
+
+
+lemma calculate_test_suite_naive_completeness :
   fixes M :: "('a::linorder,'b::linorder,'c::linorder) fsm"
   assumes "observable M" 
   and     "observable M'"
@@ -1331,18 +1311,51 @@ lemma calculate_test_suite_example_completeness :
   and     "completely_specified M"
   and     "completely_specified M'"
   and     "size M' \<le> m"
-shows     "(L M' \<subseteq> L M) \<longleftrightarrow> passes_test_suite M (calculate_test_suite_example M m) M'"
-using passes_test_suite_completeness[OF calculate_test_suite_example_sufficient_and_finite(1)[OF \<open>observable M\<close> \<open>completely_specified M\<close> \<open>inputs M \<noteq> {}\<close>, of m] assms]
-  by assumption
+shows     "(L M' \<subseteq> L M) \<longleftrightarrow> passes_test_suite M (calculate_test_suite_naive M m) M'"
+and       "(L M' \<subseteq> L M) \<longleftrightarrow> pass_io_set_maximal M' (calculate_test_suite_naive_as_io_sequences M m)"
+proof -
+
+  have  "\<And>q. q \<in> FSM.nodes M \<Longrightarrow> \<exists>d\<in>set (maximal_repetition_sets_from_separators_list_naive M). q \<in> fst d"
+    unfolding maximal_repetition_sets_from_separators_list_naive_def Let_def
+    by (metis (mono_tags, lifting) list.set_map maximal_pairwise_r_distinguishable_state_sets_from_separators_code maximal_repetition_sets_from_separators_code maximal_repetition_sets_from_separators_cover)
+  moreover have "\<And>d. d \<in> set (maximal_repetition_sets_from_separators_list_naive M) \<Longrightarrow> fst d \<subseteq> nodes M \<and> (snd d = fst d \<inter> fst ` d_reachable_states_with_preambles M)" and "\<And> d q1 q2. d \<in> set (maximal_repetition_sets_from_separators_list_naive M) \<Longrightarrow> q1\<in>fst d \<Longrightarrow> q2\<in>fst d \<Longrightarrow> q1 \<noteq> q2 \<Longrightarrow> (q1, q2) \<in> fst ` r_distinguishable_state_pairs_with_separators M"
+  proof 
+    fix d assume "d \<in> set (maximal_repetition_sets_from_separators_list_naive M)"
+    then have "d \<in> maximal_repetition_sets_from_separators M"
+      by (simp add: maximal_repetition_sets_from_separators_code_alt)
+      
+
+    then show "fst d \<subseteq> nodes M" and "(snd d = fst d \<inter> fst ` d_reachable_states_with_preambles M)" and "\<And> q1 q2 . q1\<in>fst d \<Longrightarrow> q2\<in>fst d \<Longrightarrow> q1 \<noteq> q2 \<Longrightarrow> (q1, q2) \<in> fst ` r_distinguishable_state_pairs_with_separators M"
+      unfolding maximal_repetition_sets_from_separators_def 
+                maximal_pairwise_r_distinguishable_state_sets_from_separators_def
+                pairwise_r_distinguishable_state_sets_from_separators_def 
+      by force+
+  qed
+  ultimately have "is_sufficient_for_reduction_testing (calculate_test_suite_naive M m) M m"
+             and  "is_finite_test_suite (calculate_test_suite_naive M m)"
+    using calculate_test_suite_for_repetition_sets_sufficient_and_finite[OF \<open>observable M\<close> \<open>completely_specified M\<close> \<open>inputs M \<noteq> {}\<close>]
+    unfolding calculate_test_suite_naive_def by force+
+
+  then show "(L M' \<subseteq> L M) \<longleftrightarrow> passes_test_suite M (calculate_test_suite_naive M m) M'"
+       and  "(L M' \<subseteq> L M) \<longleftrightarrow> pass_io_set_maximal M' (calculate_test_suite_naive_as_io_sequences M m)"
+    using passes_test_suite_completeness[OF _ assms] 
+          passes_test_suite_as_maximal_sequences_completeness[OF _ _ assms] 
+    unfolding calculate_test_suite_naive_as_io_sequences_def
+    by blast+
+qed
 
 
 
+subsubsection \<open>Greedy Repetition Set Strategy\<close>
 
+(* Greedily searches for one maximal pairwise r-distinguishable set for each state *)
+definition calculate_test_suite_greedy :: "('a::linorder,'b::linorder,'c::linorder) fsm \<Rightarrow> nat \<Rightarrow> ('a,'b,'c, ('a \<times> 'a) + 'a) test_suite" where
+  "calculate_test_suite_greedy M m = calculate_test_suite_for_repetition_sets M m (maximal_repetition_sets_from_separators_list_greedy M)" 
 
-definition calculate_test_suite_example_as_io_sequences :: "('a::linorder,'b::linorder,'c::linorder) fsm \<Rightarrow> nat \<Rightarrow> ('b \<times> 'c) list set" where
-  "calculate_test_suite_example_as_io_sequences M m = test_suite_to_io'_maximal M (calculate_test_suite_example M m)"
+definition calculate_test_suite_greedy_as_io_sequences :: "('a::linorder,'b::linorder,'c::linorder) fsm \<Rightarrow> nat \<Rightarrow> ('b \<times> 'c) list set" where
+  "calculate_test_suite_greedy_as_io_sequences M m = test_suite_to_io'_maximal M (calculate_test_suite_greedy M m)"
 
-lemma calculate_test_suite_example_as_io_sequences_completeness :
+lemma calculate_test_suite_greedy_completeness :
   fixes M :: "('a::linorder,'b::linorder,'c::linorder) fsm"
   assumes "observable M" 
   and     "observable M'"
@@ -1351,48 +1364,43 @@ lemma calculate_test_suite_example_as_io_sequences_completeness :
   and     "completely_specified M"
   and     "completely_specified M'"
   and     "size M' \<le> m"
-shows     "(L M' \<subseteq> L M) \<longleftrightarrow> pass_io_set_maximal M' (calculate_test_suite_example_as_io_sequences M m)"
-  unfolding calculate_test_suite_example_as_io_sequences_def
-  using passes_test_suite_as_maximal_sequences_completeness[OF calculate_test_suite_example_sufficient_and_finite[OF \<open>observable M\<close> \<open>completely_specified M\<close> \<open>inputs M \<noteq> {}\<close>, of m] assms]
-  by assumption
+shows     "(L M' \<subseteq> L M) \<longleftrightarrow> passes_test_suite M (calculate_test_suite_greedy M m) M'"
+and       "(L M' \<subseteq> L M) \<longleftrightarrow> pass_io_set_maximal M' (calculate_test_suite_greedy_as_io_sequences M m)"
+proof -
+
+  have  "\<And>q. q \<in> FSM.nodes M \<Longrightarrow> \<exists>d\<in>set (maximal_repetition_sets_from_separators_list_greedy M). q \<in> fst d"
+    unfolding maximal_repetition_sets_from_separators_list_greedy_def Let_def
+    using greedy_pairwise_r_distinguishable_state_sets_from_separators_cover[of _ M]
+    by simp 
+
+  moreover have "\<And>d. d \<in> set (maximal_repetition_sets_from_separators_list_greedy M) \<Longrightarrow> fst d \<subseteq> nodes M \<and> (snd d = fst d \<inter> fst ` d_reachable_states_with_preambles M)" and "\<And> d q1 q2. d \<in> set (maximal_repetition_sets_from_separators_list_greedy M) \<Longrightarrow> q1\<in>fst d \<Longrightarrow> q2\<in>fst d \<Longrightarrow> q1 \<noteq> q2 \<Longrightarrow> (q1, q2) \<in> fst ` r_distinguishable_state_pairs_with_separators M"
+  proof 
+    fix d assume "d \<in> set (maximal_repetition_sets_from_separators_list_greedy M)"
+    then have "fst d \<in> set (greedy_pairwise_r_distinguishable_state_sets_from_separators M)"
+         and  "(snd d = fst d \<inter> fst ` d_reachable_states_with_preambles M)"
+      unfolding maximal_repetition_sets_from_separators_list_greedy_def Let_def by force+
+
+    then have "fst d \<in> pairwise_r_distinguishable_state_sets_from_separators M"
+      using greedy_pairwise_r_distinguishable_state_sets_from_separators_soundness by blast
+    then show "fst d \<subseteq> nodes M" and "(snd d = fst d \<inter> fst ` d_reachable_states_with_preambles M)" and "\<And> q1 q2 . q1\<in>fst d \<Longrightarrow> q2\<in>fst d \<Longrightarrow> q1 \<noteq> q2 \<Longrightarrow> (q1, q2) \<in> fst ` r_distinguishable_state_pairs_with_separators M"
+      using \<open>(snd d = fst d \<inter> fst ` d_reachable_states_with_preambles M)\<close>
+      unfolding pairwise_r_distinguishable_state_sets_from_separators_def
+      by force+ 
+  qed
+  ultimately have "is_sufficient_for_reduction_testing (calculate_test_suite_greedy M m) M m"
+             and  "is_finite_test_suite (calculate_test_suite_greedy M m)"
+    using calculate_test_suite_for_repetition_sets_sufficient_and_finite[OF \<open>observable M\<close> \<open>completely_specified M\<close> \<open>inputs M \<noteq> {}\<close>]
+    unfolding calculate_test_suite_greedy_def by force+
+
+  then show "(L M' \<subseteq> L M) \<longleftrightarrow> passes_test_suite M (calculate_test_suite_greedy M m) M'"
+       and  "(L M' \<subseteq> L M) \<longleftrightarrow> pass_io_set_maximal M' (calculate_test_suite_greedy_as_io_sequences M m)"
+    using passes_test_suite_completeness[OF _ assms] 
+          passes_test_suite_as_maximal_sequences_completeness[OF _ _ assms] 
+    unfolding calculate_test_suite_greedy_as_io_sequences_def
+    by blast+
+qed
 
 
 
-
-
-
-
-
-
-
-
-
-
-subsection \<open>Examples\<close>
-
-(* TODO: move *)
-value "calculate_test_suite_example m_ex_H 4"
-value "case (calculate_test_suite_example m_ex_H 4) of
-        (Test_Suite a b c d) \<Rightarrow>
-          (image fst a,
-           image b (image fst a))"
-value "case (calculate_test_suite_example m_ex_H 4) of
-        (Test_Suite a b c d) \<Rightarrow>
-          (image (\<lambda> (x,_) . image (\<lambda> xy . (xy, c xy)) (image (Pair x) (b x))) a)"
-
-value "calculate_test_suite_example_as_io_sequences m_ex_H 4"
-value "calculate_test_suite_example_as_io_sequences m_ex_H 6"
-
-definition ex01 where "ex01 = calculate_test_suite_example_as_io_sequences m_ex_H 4"
-definition ex02 where "ex02 = calculate_test_suite_example_as_io_sequences m_ex_H 8"
-definition ex02b where "ex02b = calculate_test_suite_example_as_io_sequences m_ex_H 7"
-definition ex03 where "ex03 = calculate_test_suite_example_as_io_sequences m_ex_H 10"
-definition ex04 where "ex04 = calculate_test_suite_example_as_io_sequences m_ex_DR 4"
-definition ex05 where "ex05 = calculate_test_suite_example_as_io_sequences m_ex_DR 8"
-definition ex06 where "ex06 = calculate_test_suite_example_as_io_sequences m_ex_DR (size m_ex_DR)"
-
-(*
-export_code ex01 ex02 ex02b ex03 ex04 ex05 ex06 in Haskell module_name FSM4o
-*)
 
 end
